WIP; merge with CRIS main & working on worlds

iris_system/World.v
@@ -3,15 +3,14 @@ Require Import sflib.
 From iris.algebra Require Import ofe auth agree coPset gset gmap_view.
 From CRIS.algebra Require Import functions.
 From iris Require Import bi.big_op.
-
-Require Import Coqlib PCM IPM sProp.
+Require Import Coqlib.
+Require Export SRF sProp own.
 
 Local Notation univ_id := positive.
 Local Notation level := nat.
 
-Section INDEXED_INVARIANT_SET.
-
-  Context `{_W : CtxSL.t}.
+Section invariants.
+  Context `{α : SRFCons.t}.
 
   Canonical Structure SynO n : ofe := leibnizO (SRFSyn.t n).
 
@@ -23,148 +22,159 @@ Section INDEXED_INVARIANT_SET.
   Global Instance discrete_fun_singleton_proper' (x : univ_id) :
     Proper
       ((≡) ==> (≡))
-      (discrete_fun_singleton (B:=(λ _, discrete_funUR InvSetRA)) x).
+      (discrete_fun_singleton (B := (λ _, discrete_funUR InvSetRA)) x).
   Proof.
-    intros x1 x2 H u. destruct (decide (u = x)); last first.
+    intros x1 x2 H' u. destruct (decide (u = x)); last first.
     { rewrite ! discrete_fun_lookup_singleton_ne; eauto. }
     clarify; rewrite ! discrete_fun_lookup_singleton; eauto.
   Qed.
 
-  Definition OwnIRA : ucmra :=
+  Definition ownIRA : ucmra :=
     univ_id -d> (discrete_funUR InvSetRA).
 
-  Definition OwnERA : ucmra :=
+  Definition ownERA : ucmra :=
     univ_id -d> coPset_disjUR.
 
-  Definition OwnDRA : ucmra :=
+  Definition ownDRA : ucmra :=
     univ_id -d> (authUR (gset_disjUR positive)).
 
-End INDEXED_INVARIANT_SET.
+  Class invGpreSΣ (Σ : GRA) := {
+    invGS_I : inG ownIRA Σ
+  }.
+  Class invGpreSΓ (Γ : GRA) := {
+    invGS_E : inG ownERA Γ;
+    invGS_D : inG ownDRA Γ;
+  }.
 
-Section PCM_OWN.
+  (* Two classes for Σ and Γ are separately defined for creating syntactic wsats in sWorld.v *)
+  Class invGSΣ (Σ : GRA) := {
+    inv_preΣ : invGpreSΣ Σ;
+    invariant_name : gname;
+  }.
+  Class invGSΓ (Γ : GRA) := {
+    inv_preΓ : invGpreSΓ Γ;
+    enabled_name : gname;
+    disabled_name : gname;
+  }.
 
-  Context `{_W : CtxSL.t}.
-  Context `{@GRA.inG OwnIRA Σ}.
+  Class invGS (Σ Γ : GRA) := {
+    #[global] invGS_Σ :: invGSΣ Σ;
+    #[global] invGS_Γ :: invGSΓ Γ;
+  }.
 
-  (* Owns invariant *)
-  Definition OwnIR (u : univ_id) (n : level) (i : positive) (p : SRFSyn.t n) : OwnIRA :=
+  Definition invΣ : GRA := #[[ownIRA]].
+  Definition invΓ : GRA := #[[ownERA]; [ownDRA]].
+
+  Global Instance subG_invΣ {Σ} : subG invΣ Σ → invGpreSΣ Σ.
+  Proof. solve_inG. Qed.
+  Global Instance subG_invΓ {Γ} : subG invΓ Γ → invGpreSΓ Γ.
+  Proof. solve_inG. Qed.
+End invariants.
+
+Section predicates.
+  Context `{!CtxSL.t Σ Γ α β τ, !invGS Σ Γ}.
+  Local Existing Instances inv_preΣ inv_preΓ invGS_I invGS_E invGS_D.
+
+  (* owns invariant *)
+  Definition ownIR (u : univ_id) (n : level) (i : positive) (p : SRFSyn.t n) : ownIRA :=
     discrete_fun_singleton u
       (discrete_fun_singleton n
         (gmap_view_frag i DfracDiscarded (to_agree p))).
-  Definition OwnI (u : univ_id) (n : level) (i : positive) (p : SRFSyn.t n) :=
-    OwnM (OwnIR u n i p).
+  Definition ownI (u : univ_id) (n : level) (i : positive) (p : SRFSyn.t n) : iProp Σ :=
+    own invariant_name (ownIR u n i p).
 
-  Definition OwnI_authR (u : univ_id) (n : level) (I : gmap positive (SRFSyn.t n)) : OwnIRA :=
+  Global Instance ownI_persistent
+    u n i p : Persistent (ownI u n i p).
+  Proof. apply _. Qed.
+
+  Definition ownI_authR (u : univ_id) (n : level) (I : gmap positive (SRFSyn.t n)) : ownIRA :=
     discrete_fun_singleton u
       (discrete_fun_singleton n
         (gmap_view_auth (DfracOwn 1) (to_agree <$> I))).
-  Definition OwnI_auth (u : univ_id) (n : level) (I : gmap positive (SRFSyn.t n)) :=
-    OwnM (OwnI_authR u n I).
+  Definition ownI_auth (u : univ_id) (n : level) (I : gmap positive (SRFSyn.t n)) :=
+    own invariant_name (ownI_authR u n I).
 
-  Context `{@GRA.inG OwnERA Γ}.
-
-  Definition OwnER (u : univ_id) (E : coPset) : OwnERA :=
+  Definition ownER (u : univ_id) (E : coPset) : ownERA :=
     discrete_fun_singleton u (CoPset E).
-  Definition OwnE (u : univ_id) (E : coPset) : iProp Σ :=
-    OwnM (OwnER u E).
+  Definition ownE (u : univ_id) (E : coPset) : iProp Σ :=
+    own enabled_name (ownER u E).
 
-  Context `{@GRA.inG OwnDRA Γ}.
-
-  Definition OwnDR (u : univ_id) (D : gset positive) : OwnDRA :=
+  Definition ownDR (u : univ_id) (D : gset positive) : ownDRA :=
     discrete_fun_singleton u (◯ (GSet D)).
-  Definition OwnD (u : univ_id) (D : gset positive) :=
-    OwnM (OwnDR u D).
+  Definition ownD (u : univ_id) (D : gset positive) : iProp Σ :=
+    own disabled_name (ownDR u D).
 
-  Definition OwnD_authR  (u : univ_id) (D : gset positive) : OwnDRA :=
+  Definition ownD_authR  (u : univ_id) (D : gset positive) : ownDRA :=
     discrete_fun_singleton u (● (GSet D)).
-  Definition OwnD_auth (u : univ_id) : iProp Σ :=
-    (∃ D, OwnM (OwnD_authR u D))%I.
+  Definition ownD_auth (u : univ_id) : iProp Σ :=
+    ∃ D, own disabled_name (ownD_authR u D).
 
-  Lemma OwnE_exploit u (E1 E2 : coPset) :
-    OwnE u E1 ∗ OwnE u E2 ⊢ ⌜E1 ## E2⌝.
+  Lemma ownE_exploit u (E1 E2 : coPset) :
+    ownE u E1 ∗ ownE u E2 ⊢ ⌜E1 ## E2⌝.
   Proof.
     iIntros "[H1 H2]". iCombine "H1 H2" gives %WF.
     by rewrite discrete_fun_singleton_op discrete_fun_singleton_valid coPset_disj_valid_op in WF.
   Qed.
 
-  Lemma OwnE_union u (E1 E2 : coPset) :
-    OwnE u E1 ∗ OwnE u E2 ⊢ OwnE u (E1 ∪ E2).
+  Lemma ownE_op u (E1 E2 : coPset) :
+    E1 ## E2 → ownE u E1 ∗ ownE u E2 ⊣⊢ ownE u (E1 ∪ E2).
   Proof.
-    iIntros "H". iDestruct (OwnE_exploit with "H") as %D.
-    rewrite -OwnM_op discrete_fun_singleton_op coPset_disj_union //.
+    intros dis; rewrite -own_op discrete_fun_singleton_op coPset_disj_union; ss.
   Qed.
 
-  Lemma OwnE_disjoint u (E1 E2 : coPset) :
-    E1 ## E2 -> OwnE u (E1 ∪ E2) ⊢ OwnE u E1 ∗ OwnE u E2.
-  Proof.
-    iIntros (D) "H".
-    rewrite /OwnE -OwnM_op discrete_fun_singleton_op coPset_disj_union //.
-  Qed.
-
-  Lemma OwnE_subset u (E1 E2 : coPset) :
-    E1 ⊆ E2 -> OwnE u E2 ⊢ OwnE u E1 ∗ (OwnE u E1 -∗ OwnE u E2).
+  Lemma ownE_subset u (E1 E2 : coPset) :
+    E1 ⊆ E2 -> ownE u E2 ⊢ ownE u E1 ∗ (ownE u E1 -∗ ownE u E2).
   Proof.
     iIntros (SUB) "E".
     rewrite (union_difference_L E1 E2); [|done].
-    iPoseProof (OwnE_disjoint with "E") as "[E1 E2]"; [set_solver|].
+    iPoseProof (ownE_op with "E") as "[E1 E2]"; [set_solver|].
     iFrame. iIntros "E1".
-    iApply OwnE_union. iFrame.
+    iApply ownE_op; [set_solver|iFrame].
   Qed.
+End predicates.
 
-  Global Instance OwnI_persistent
-    u n i p : Persistent (OwnI u n i p).
-  Proof. apply _. Qed.
-
-End PCM_OWN.
-
-Section WORLD_SATISFACTION.
-
-  Context `{_W : CtxSL.t}.
-  Context `{_W0 : @GRA.inG OwnIRA Σ}.
-  Context `{_W1 : @GRA.inG OwnERA Γ}.
-  Context `{_W2 : @GRA.inG OwnDRA Γ}.
-  Notation iProp := (iProp Σ).
+Section wsat.
+  Context `{!CtxSL.t Σ Γ α β τ, !invGS Σ Γ}.
 
   Variable u : univ_id.
   Variable n : level.
 
+  Definition inv_satall (I : gmap positive (SRFSyn.t n)) : iProp Σ :=
+    [∗ map] i ↦ p ∈ I, (⟦p⟧ ∗ ownD u {[i]}) ∨ ownE u {[i]}.
 
-  Definition inv_satall (I : gmap positive (SRFSyn.t n)) : iProp :=
-    [∗ map] i ↦ p ∈ I, (⟦p⟧ ∗ OwnD u {[i]}) ∨ OwnE u {[i]}.
-
-  Definition wsat : iProp := (∃ I, OwnI_auth u n I ∗ inv_satall I)%I.
+  Definition wsat : iProp Σ := ∃ I, ownI_auth u n I ∗ inv_satall I.
 
   Lemma alloc_name φ (INF : pred_infinite φ) :
-    OwnD_auth u ⊢ |==> OwnD_auth u ∗ ∃ i, ⌜φ i⌝ ∧ OwnD u {[i]}.
+    ownD_auth u ⊢ |==> ownD_auth u ∗ ∃ i, ⌜φ i⌝ ∧ ownD u {[i]}.
   Proof.
     iIntros "[% DA]".
     rewrite (pred_infinite_set φ (C:=gset univ_id)) in INF.
     hexploit (INF D); intros [x [??]].
-    iPoseProof (OwnM_Upd with "DA") as "> DA".
+    iPoseProof (own_update with "DA") as "> DA".
     { by eapply discrete_fun_singleton_update, auth_update_alloc,
         gset_disj_alloc_empty_local_update, disjoint_singleton_l.
     }
-    iEval (rewrite -discrete_fun_singleton_op) in "DA"; iPoseProof (OwnM_op with "DA") as "[D1 D2]".
+    iEval (rewrite -discrete_fun_singleton_op) in "DA"; iPoseProof (own_op with "DA") as "[D1 D2]".
     iModIntro; iSplitL "D1"; iFrame.
     iPureIntro; done.
   Qed.
 
-  Lemma wsat_OwnI_alloc_gen p φ (INF : pred_infinite φ) :
-    OwnD_auth u ∗ wsat ⊢ |==> (∃ i, ⌜φ i⌝ ∧ OwnI u n i p) ∗ OwnD_auth u ∗ (⟦p⟧ -∗ wsat).
+  Lemma wsat_ownI_alloc_gen p φ (INF : pred_infinite φ) :
+    ownD_auth u ∗ wsat ⊢ |==> (∃ i, ⌜φ i⌝ ∧ ownI u n i p) ∗ ownD_auth u ∗ (⟦p⟧ -∗ wsat).
   Proof.
-    iIntros "[DA [%I [IA INV]]]"; rewrite /OwnI_auth /inv_satall.
+    iIntros "[DA [%I [IA INV]]]"; rewrite /ownI_auth /inv_satall.
     iMod (alloc_name (λ i, φ i ∧ i ∉ dom I) with "DA") as "[DA [% [% D]]]".
     { intros l; hexploit (INF (l ++ (elements (dom I)))); intros [x [H1 H2]]; exists x.
       eapply not_elem_of_app in H2; des; repeat split; eauto.
       rewrite elem_of_elements in H0; eauto.
     }
-    iPoseProof (OwnM_Upd with "IA") as "> IA".
+    iPoseProof (own_update with "IA") as "> IA".
     { do 2 eapply discrete_fun_singleton_update.
       eapply (gmap_view_alloc (to_agree <$> I) i (DfracOwn 1) (to_agree (A:=leibnizO _) p)); ss.
       eapply not_elem_of_dom; rewrite dom_fmap_L; des; eauto.
     }
-    rewrite -?discrete_fun_singleton_op; iPoseProof (OwnM_op with "IA") as "[I1 I2]".
-    iMod (OwnM_Upd with "I2") as "I2".
+    rewrite -?discrete_fun_singleton_op; iPoseProof (own_op with "IA") as "[I1 I2]".
+    iMod (own_update with "I2") as "I2".
     { do 2 eapply discrete_fun_singleton_update; eapply gmap_view_frag_persist. }
     iModIntro; iFrame; iSplit; [iPureIntro; des; ss|iIntros "P"].
     iExists (<[i:=p]> I); iSplitL "I1".
@@ -174,23 +184,23 @@ Section WORLD_SATISFACTION.
     iFrame. iLeft; iFrame.
   Qed.
 
-  Lemma wsat_OwnI_alloc p φ (INF : pred_infinite φ) :
-    OwnD_auth u ∗ wsat ∗ ⟦p⟧ ⊢ |==> (∃ i, ⌜φ i⌝ ∧ OwnI u n i p) ∗ OwnD_auth u ∗ wsat.
+  Lemma wsat_ownI_alloc p φ (INF : pred_infinite φ) :
+    ownD_auth u ∗ wsat ∗ ⟦p⟧ ⊢ |==> (∃ i, ⌜φ i⌝ ∧ ownI u n i p) ∗ ownD_auth u ∗ wsat.
   Proof.
     iIntros "(D & W & P)".
-    iMod (wsat_OwnI_alloc_gen with "[D W]") as "(I & D & W)". eauto. iFrame.
+    iMod (wsat_ownI_alloc_gen with "[D W]") as "(I & D & W)". eauto. iFrame.
     iFrame. iModIntro. iApply "W". iFrame.
   Qed.
 
-  Lemma wsat_OwnI_open i p :
-    OwnI u n i p ∗ wsat ∗ OwnE u {[i]} ⊢ |==> ⟦p⟧ ∗ wsat ∗ OwnD u {[i]}.
+  Lemma wsat_ownI_open i p :
+    ownI u n i p ∗ wsat ∗ ownE u {[i]} ⊢ |==> ⟦p⟧ ∗ wsat ∗ ownD u {[i]}.
   Proof.
     iIntros "(I & [% [AUTH SAT]] & EN)". iModIntro.
-    iCombine "AUTH I" as "AUTH"; iPoseProof (OwnM_valid with "AUTH") as "%WF".
+    iCombine "AUTH I" as "AUTH"; iPoseProof (own_valid with "AUTH") as "%WF".
     rewrite ?discrete_fun_singleton_op ?discrete_fun_singleton_valid in WF.
     eapply gmap_view_both_dfrac_valid_discrete_total in WF; des.
     eapply lookup_fmap_Some in WF1; des; clarify.
-    hexploit (to_agree_included p x); eauto; intros H; apply H in WF3; inv WF3.
+    hexploit (to_agree_included p x); eauto; intros Hin; apply Hin in WF3; inv WF3.
     iDestruct "AUTH" as "[AUTH I]".
     iPoseProof (big_sepM_delete with "SAT") as "[[[H1 H2]|H1] SAT]"; eauto.
     { iPoseProof (big_sepM_insert _ (delete i I) i x with "[SAT EN]") as "SAT".
@@ -198,22 +208,22 @@ Section WORLD_SATISFACTION.
       { iFrame. iRight; iFrame. }
       rewrite insert_delete; eauto. iFrame.
     }
-    iPoseProof (OwnE_exploit with "[EN H1]") as "%"; iFrame; set_solver.
+    iPoseProof (ownE_exploit with "[EN H1]") as "%"; iFrame; set_solver.
   Qed.
 
-  Lemma wsat_OwnI_close i p :
-    OwnI u n i p ∗ wsat ∗ ⟦p⟧ ∗ OwnD u {[i]} ⊢ |==> wsat ∗ OwnE u {[i]}.
+  Lemma wsat_ownI_close i p :
+    ownI u n i p ∗ wsat ∗ ⟦p⟧ ∗ ownD u {[i]} ⊢ |==> wsat ∗ ownE u {[i]}.
   Proof.
     iIntros "(I & [% [AUTH SAT]] & P & DIS)". iModIntro.
-    iCombine "AUTH I" as "AUTH"; iPoseProof (OwnM_valid with "AUTH") as "%WF".
+    iCombine "AUTH I" as "AUTH"; iPoseProof (own_valid with "AUTH") as "%WF".
     rewrite ?discrete_fun_singleton_op ?discrete_fun_singleton_valid in WF.
     eapply gmap_view_both_dfrac_valid_discrete_total in WF; des.
     eapply lookup_fmap_Some in WF1; des; clarify.
-    hexploit (to_agree_included p x); eauto; intros H; apply H in WF3; inv WF3.
+    hexploit (to_agree_included p x); eauto; intros Hin; apply Hin in WF3; inv WF3.
     iDestruct "AUTH" as "[AUTH I]".
     iPoseProof (big_sepM_delete with "SAT") as "[[[H1 H2]|H1] SAT]"; eauto.
     { iCombine "DIS H2" as "F". rewrite discrete_fun_singleton_op.
-      iPoseProof (OwnM_valid with "F") as "%WF'".
+      iPoseProof (own_valid with "F") as "%WF'".
       rewrite discrete_fun_singleton_valid auth_frag_op_valid gset_disj_valid_op in WF'; set_solver.
     }
     iPoseProof (big_sepM_insert _ (delete i I) i x with "[SAT P DIS]") as "SAT".
@@ -223,13 +233,12 @@ Section WORLD_SATISFACTION.
   Qed.
 
   Lemma wsat_init :
-    OwnI_auth u n ∅ ⊢ wsat.
+    ownI_auth u n ∅ ⊢ wsat.
   Proof.
     iIntros "H"; iExists ∅; iFrame; iApply big_sepM_empty; ss.
   Qed.
-
-End WORLD_SATISFACTION.
-
+End wsat.
+(* 
 Section UNIVERSE.
 
   Fixpoint pos_sup (p i : positive) : bool :=
@@ -313,55 +322,104 @@ Section UNIVERSE.
     revert_until u. induction u; i; destruct k; ss; eauto.
   Qed.
 
-End UNIVERSE.
+End UNIVERSE. *)
 
 Section WSATS.
+  Context `{!CtxSL.t Σ Γ α β τ, !invGS Σ Γ}.
+  Local Existing Instances inv_preΣ inv_preΓ invGS_I invGS_E invGS_D.
 
-  Context `{_W : CtxSL.t}.
-  Context `{_W0 : @GRA.inG OwnIRA Σ}.
-  Context `{_W1 : @GRA.inG OwnERA Γ}.
-  Context `{_W2 : @GRA.inG OwnDRA Γ}.
-  Notation iProp := (iProp Σ).
-
-  Definition free_worldsR u b : OwnIRA :=
+  Definition wsat_authR u b : ownIRA :=
     discrete_fun_singleton u
       ((λ n, if (n <? b) then ε else gmap_view_auth (DfracOwn 1) ∅) : discrete_funUR InvSetRA).
-  Definition free_worlds u b := OwnM (free_worldsR u b).
+  Definition wsat_auth u b : iProp Σ := own invariant_name (wsat_authR u b).
 
-  Definition empty_universesR {R : univ_id -> ucmra} eu (r : forall u, R u) : discrete_funUR R :=
+  (* Definition empty_universesR {R : univ_id -> ucmra} eu (r : forall u, R u) : discrete_funUR R :=
     fun u =>
       if (eu <? u)%positive
       then r u
       else ε.
-  Definition empty_universes (eu : univ_id) : iProp :=
-    OwnM (empty_universesR eu (λ _, CoPset ⊤))
-    ∗ OwnM (empty_universesR eu (λ _, ● (GSet ∅)))
-    ∗ OwnM (empty_universesR eu (λ _, (λ n, gmap_view_auth (DfracOwn 1) ∅) : discrete_funUR InvSetRA)).
-  Definition free_universes := (∃ eu, empty_universes eu)%I.
+  Definition empty_universes (eu : univ_id) : iProp Σ :=
+    own enabled_name (empty_universesR eu (λ _, CoPset ⊤))
+    ∗ own disabled_name (empty_universesR eu (λ _, ● (GSet ∅)))
+    ∗ own invariant_name (empty_universesR eu ((λ _, (λ n, gmap_view_auth (DfracOwn 1) ∅)) : ownIRA)). *)
+  (* Definition free_universes := (∃ eu, empty_universes eu)%I. *)
 
-  Definition wsats u b : iProp := ([∗ list] n ∈ (seq 0 b), wsat u n)%I.
-  Definition used_worlds u b E : iProp :=
-    wsats u b ∗ OwnE u E ∗ OwnD_auth u ∗ free_universes.
-  Definition closed_universe u b E : iProp :=
-    used_worlds u b E ∗ free_worlds u b.
+  Definition wsats u b E : iProp Σ :=
+    wsat_auth u b ∗ ownE u E ∗ ownD_auth u ∗ [∗ list] n ∈ (seq 0 b), wsat u n.
 
-  Lemma wsats_fold u b :
+  Local Definition uPred_fupd_def u b (E1 E2 : coPset) (P : iProp Σ) : iProp Σ :=
+    wsats u b E1 ==∗ (wsats u b E2 ∗ P).
+  Local Definition uPred_fupd_aux : seal (@uPred_fupd_def). Proof. by eexists. Qed.
+  Definition uPred_fupd := uPred_fupd_aux.(unseal).
+  Local Definition uPred_fupd_eq : @uPred_fupd = @uPred_fupd_def := uPred_fupd_aux.(seal_eq).
+  Local Lemma uPred_fupd_unseal u b : @fupd _ (uPred_fupd u b) = (uPred_fupd_def u b).
+  Proof. rewrite -uPred_fupd_eq //. Qed.
+
+  Lemma uPred_fupd_mixin u n : BiFUpdMixin (iProp Σ) (uPred_fupd u n).
+  Proof.
+    split.
+    - rewrite /updates.fupd uPred_fupd_eq. solve_proper.
+    - intros E1 E2 (E1''&->&?)%subseteq_disjoint_union_L.
+      rewrite /fupd uPred_fupd_eq /uPred_fupd_def /wsats -ownE_op //.
+      by iIntros "($ & ($ & $) & $ & $) !> ($ & $ & $ & $) !>".
+    - rewrite /fupd uPred_fupd_eq /uPred_fupd_def /wsats /bi_except_0.
+      iIntros (E1 E2 P) "[H | H]"; iFrame.
+      iDestruct (uPred.later_eq with "H") as "H"; by iFrame.
+    - rewrite /fupd uPred_fupd_eq /uPred_fupd_def /wsats.
+      iIntros (E1 E2 P Q HPQ) "HP HwE". rewrite -HPQ. by iApply "HP".
+    - rewrite /fupd uPred_fupd_eq /uPred_fupd_def /wsats. iIntros (E1 E2 E3 P) "HP HwE".
+      iMod ("HP" with "HwE") as "(HA & HP)". iApply "HP"; by iFrame.
+    - intros E1 E2 Ef P HE1Ef. rewrite /fupd uPred_fupd_eq /uPred_fupd_def /wsats -ownE_op //.
+      iIntros "Hupd (AUTH & [E1 Ef] & D & WSAT)".
+      iMod ("Hupd" with "[AUTH E1 D WSAT]") as "[($ & E2 & $ & $) P]"; iFrame.
+      iPoseProof (ownE_exploit with "[Ef E2]") as "%DISJ"; first iFrame.
+      iModIntro; rewrite -ownE_op //=.
+      iFrame. iApply "P"; done.
+    - rewrite /fupd uPred_fupd_eq /uPred_fupd_def /wsats. by iIntros (????) "[HwP $]".
+  Qed.
+  Global Instance uPred_bi_fupd u n : BiFUpd (iProp Σ) :=
+    {| bi_fupd_mixin := (uPred_fupd_mixin u n) |}.
+  Global Instance uPred_bi_bupd_fupd u n :
+    @BiBUpdFUpd (iProp Σ) (uPred_bi_bupd Σ) (uPred_bi_fupd u n).
+  Proof. rewrite /BiBUpdFUpd uPred_fupd_unseal. by iIntros (E P) ">? [$ $] !>". Qed.
+
+  Notation fupd_ex u n :=
+    (@fupd (bi_car (uPredI (GRAUR Σ))) (@bi_fupd_fupd _ (uPred_bi_fupd u n))) (only parsing).
+
+  Notation "'=|' u ',' n '|={' E1 ',' E2 '}=>' P" := (fupd_ex u n E1 E2 P)%I (at level 90).
+  Notation "P '=|' u ',' n '|={' E1 ',' E2 '}=∗' Q" := (P -∗ =|u, n|={E1,E2}=> Q)%I (at level 90).
+
+  Notation "'=|' u ',' n '|={' E '}=>' P" := (=|u, n|={E, E}=> P)%I (at level 90).
+  Notation "P '=|' u ',' n '|={' E '}=∗' Q" := (P -∗ =|u, n|={E, E}=> Q)%I (at level 90).
+
+  Local Definition inv_def u (n : level) (N : namespace) (p : SRFSyn.t n) : iProp Σ :=
+    ∃ i, ⌜i ∈ (↑N : coPset)⌝ ∧ ownI u n i p.
+  Local Definition inv_aux : seal (@inv_def). Proof. by eexists. Qed.
+  Definition inv := inv_aux.(unseal).
+  Local Definition inv_eq : @inv = @inv_def := inv_aux.(seal_eq).
+
+  (* Definition used_worlds u b E : iProp Σ :=
+    wsats u b ∗ ownE u E ∗ ownD_auth u ∗ free_universes. *)
+  (* Definition closed_universe u b E : iProp Σ :=
+    used_worlds u b E ∗ wsat_auth u b. *)
+
+  (* Lemma wsats_fold u b :
     wsats u (S b) ⊣⊢ (wsat u b ∗ wsats u b)%I.
   Proof.
     iSplit; replace (S b) with (b + 1) by lia; rewrite /wsats (seq_app b 1 0); ss;
       iIntros; by rewrite big_sepL_app big_sepL_singleton comm.
-  Qed.
+  Qed. *)
 
-  Lemma free_worlds_alloc u (b b' : level) (NIN : b < b') :
-    free_worlds u b ⊢ free_worlds u b' ∗ ([∗ list] n ∈ (seq b (b' - b)), wsat u n).
+  (* Lemma free_worlds_alloc u (b b' : level) (NIN : b < b') :
+    wsat_auth u b ⊢ wsat_auth u b' ∗ ([∗ list] n ∈ (seq b (b' - b)), wsat u n).
   Proof.
-    rewrite /free_worlds /free_worldsR.
+    rewrite /wsat_auth /wsat_authR.
     induction NIN; iIntros "FW".
     { replace (S b - b) with 1 by lia; ss.
       iEval (rewrite (discrete_fun_delete b (λ n, if n <? b then ε else gmap_view_auth (DfracOwn 1) ∅))) in "FW".
-      rewrite -discrete_fun_singleton_op OwnM_op. des_ifs; first by rewrite Nat.ltb_lt in Heq; lia.
+      rewrite -discrete_fun_singleton_op own_op. des_ifs; first by rewrite Nat.ltb_lt in Heq; lia.
       iDestruct "FW" as "[FW1 FW2]"; iSplitL "FW1"; last iSplitL; [|iApply wsat_init; iFrame|eauto].
-      iPoseProof (OwnM_extends with "FW1") as "?"; last iFrame.
+      iPoseProof (ownM_extends with "FW1") as "?"; last iFrame.
       exists ε; rewrite right_id; intros i; destruct (decide (i = u)); clarify;
         [rewrite !discrete_fun_lookup_singleton|rewrite !discrete_fun_lookup_singleton_ne]; eauto.
       intros x; ss; des_ifs. 
@@ -371,10 +429,10 @@ Section WSATS.
     }
     { iPoseProof (IHNIN with "FW") as "FW".
       iEval (rewrite (discrete_fun_delete m (λ n, if n <? m then ε else gmap_view_auth (DfracOwn 1) ∅))) in "FW".
-      rewrite -discrete_fun_singleton_op OwnM_op. des_ifs; first by rewrite Nat.ltb_lt in Heq; lia.
+      rewrite -discrete_fun_singleton_op own_op. des_ifs; first by rewrite Nat.ltb_lt in Heq; lia.
       iDestruct "FW" as "[[FW1 FW2] FW3]"; iPoseProof (wsat_init with "FW2") as "FW2".
       iSplitR "FW2 FW3".
-      { iPoseProof (OwnM_extends with "FW1") as "?"; last iFrame.
+      { iPoseProof (ownM_extends with "FW1") as "?"; last iFrame.
         exists ε; rewrite right_id; intros i; destruct (decide (i = u)); clarify;
           [rewrite !discrete_fun_lookup_singleton|rewrite !discrete_fun_lookup_singleton_ne]; eauto.
         intros x; ss; des_ifs. 
@@ -393,10 +451,10 @@ Section WSATS.
   Proof.
     replace b' with (b + (b' - b)) at 2 by lia.
     rewrite /wsats (seq_app b _) /= big_sepL_app; eauto.
-  Qed.
+  Qed. *)
 
  (* Lemma free_worlds_nin u (b b' : level) (LE : b <= b')
-    : free_worlds u b ⊢ free_worlds u b' ∗
+    : wsat_auth u b ⊢ wsat_auth u b' ∗
                       ([∗ list] n ∈ (seq b (b' - b)), wsat u n).
   Proof.
     iIntros "R".
@@ -406,25 +464,25 @@ Section WSATS.
   Qed.
 
   Lemma wsats_allocs u b b':
-    b <= b' -> free_worlds u b ∗ wsats u b ⊢ free_worlds u b' ∗ wsats u b'.
+    b <= b' -> wsat_auth u b ∗ wsats u b ⊢ wsat_auth u b' ∗ wsats u b'.
   Proof.
     iIntros (LE) "(AUTH & SAT)".
     iPoseProof ((free_worlds_nin _ _ _ LE) with "AUTH") as "(AUTH & NEW)". iFrame.
     iPoseProof ((wsats_nin _ _ _ LE) with "[SAT NEW]") as "SAT". iFrame. iFrame.
   Qed.
 
-  Lemma wsats_OwnI_alloc_lt_gen u n b (IN : n < b) p φ
+  Lemma wsats_ownI_alloc_lt_gen u n b (IN : n < b) p φ
         (INF : forall (E : level -> option (gset positive)) n,
             match E n with
             | None => True
             | Some G => (exists i, i ∉ G /\ φ i)
             end)
-    : OwnD_auth u ∗ wsats u b ⊢ |==> (∃ i, ⌜φ i⌝ ∧ OwnI u n i p) ∗ OwnD_auth u ∗ (⟦p⟧ -∗ wsats u b).
+    : ownD_auth u ∗ wsats u b ⊢ |==> (∃ i, ⌜φ i⌝ ∧ ownI u n i p) ∗ ownD_auth u ∗ (⟦p⟧ -∗ wsats u b).
   Proof.
     iIntros "[DA SALL]". iPoseProof (wsats_unfold with "SALL") as "SALL".
     iPoseProof (big_sepL_lookup_acc with "SALL") as "[WSAT K]".
     { apply lookup_seq_lt; eauto. }
-    iPoseProof (wsat_OwnI_alloc_gen with "[DA WSAT]") as ">(RES & DA & WSAT)".
+    iPoseProof (wsat_ownI_alloc_gen with "[DA WSAT]") as ">(RES & DA & WSAT)".
     { apply INF. } { iFrame. }
     iFrame. iModIntro. iIntros "P".
     iPoseProof ("WSAT" with "P") as "WSAT".
@@ -432,59 +490,59 @@ Section WSATS.
     iApply wsats_fold. iFrame.
   Qed.
 
-  Lemma wsats_OwnI_alloc_lt u n b (IN : n < b) p φ
+  Lemma wsats_ownI_alloc_lt u n b (IN : n < b) p φ
         (INF : forall (E : level -> option (gset positive)) n,
             match E n with
             | None => True
             | Some G => (exists i, i ∉ G /\ φ i)
             end)
-    : OwnD_auth u ∗ wsats u b ∗ ⟦p⟧ ⊢
-        |==> (∃ i, ⌜φ i⌝ ∧ OwnI u n i p) ∗ OwnD_auth u ∗ wsats u b.
+    : ownD_auth u ∗ wsats u b ∗ ⟦p⟧ ⊢
+        |==> (∃ i, ⌜φ i⌝ ∧ ownI u n i p) ∗ ownD_auth u ∗ wsats u b.
   Proof.
     iIntros "(D & W & P)".
-    iMod (wsats_OwnI_alloc_lt_gen with "[D W]") as "(I & D & W)"; eauto. iFrame.
+    iMod (wsats_ownI_alloc_lt_gen with "[D W]") as "(I & D & W)"; eauto. iFrame.
     iModIntro. iFrame. iApply "W". iFrame.
   Qed.
 
-  Lemma wsats_OwnI_alloc_ge_gen u b n (GE : b <= n) p φ
+  Lemma wsats_ownI_alloc_ge_gen u b n (GE : b <= n) p φ
         (INF : forall (E : level -> option (gset positive)) n,
             match E n with
             | None => True
             | Some G => (exists i, i ∉ G /\ φ i)
             end)
-    : free_worlds u b ∗ OwnD_auth u ∗ wsats u b ⊢
-        |==> ((∃ i, ⌜φ i⌝ ∧ OwnI u n i p)
-              ∗ free_worlds u (S n) ∗ OwnD_auth u ∗ (⟦p⟧ -∗ wsats u (S n))).
+    : wsat_auth u b ∗ ownD_auth u ∗ wsats u b ⊢
+        |==> ((∃ i, ⌜φ i⌝ ∧ ownI u n i p)
+              ∗ wsat_auth u (S n) ∗ ownD_auth u ∗ (⟦p⟧ -∗ wsats u (S n))).
   Proof.
     iIntros "(AUTH & D & WSAT)".
     iPoseProof ((wsats_allocs u b (S n)) with "[AUTH WSAT]") as "[AUTH WSAT]". lia. iFrame.
-    iMod ((wsats_OwnI_alloc_lt_gen u n (S n)) with "[D WSAT]") as "[RES WSAT]". auto. eauto. iFrame.
+    iMod ((wsats_ownI_alloc_lt_gen u n (S n)) with "[D WSAT]") as "[RES WSAT]". auto. eauto. iFrame.
     iModIntro. iFrame.
   Qed.
 
-  Lemma wsats_OwnI_alloc_ge u b n (GE : b <= n) p φ
+  Lemma wsats_ownI_alloc_ge u b n (GE : b <= n) p φ
         (INF : forall (E : level -> option (gset positive)) n,
             match E n with
             | None => True
             | Some G => (exists i, i ∉ G /\ φ i)
             end)
-    : free_worlds u b ∗ OwnD_auth u ∗ wsats u b ∗ ⟦p⟧ ⊢
-        |==> ((∃ i, ⌜φ i⌝ ∧ OwnI u n i p)
-                ∗ free_worlds u (S n) ∗ OwnD_auth u ∗ wsats u (S n)).
+    : wsat_auth u b ∗ ownD_auth u ∗ wsats u b ∗ ⟦p⟧ ⊢
+        |==> ((∃ i, ⌜φ i⌝ ∧ ownI u n i p)
+                ∗ wsat_auth u (S n) ∗ ownD_auth u ∗ wsats u (S n)).
   Proof.
-    iIntros "(A & D & W & P)". iMod (wsats_OwnI_alloc_ge_gen with "[A D W]") as "(I & A & D & W)".
+    iIntros "(A & D & W & P)". iMod (wsats_ownI_alloc_ge_gen with "[A D W]") as "(I & A & D & W)".
     1,2 : eauto. iFrame.
     iFrame. iModIntro. iFrame. iApply "W". iFrame.
   Qed.
 
-  Lemma free_worlds_OwnI_le u b n i p :
-    OwnI u n i p ∗ free_worlds u b ⊢ ⌜n < b⌝.
+  Lemma free_worlds_ownI_le u b n i p :
+    ownI u n i p ∗ wsat_auth u b ⊢ ⌜n < b⌝.
   Proof.
     iIntros "(I & AUTH)".
-    unfold OwnI, free_worlds, free_worlds.
+    unfold ownI, wsat_auth, wsat_auth.
     iCombine "AUTH I" as "AUTH".
-    iPoseProof (OwnM_valid with "AUTH") as "%WF".
-    unfold free_worldsR, OwnIR, maps_to_res, maps_to_res_dep in WF.
+    iPoseProof (own_valid with "AUTH") as "%WF".
+    unfold wsat_authR, ownIR, maps_to_res, maps_to_res_dep in WF.
     unfold URA.add in WF. unseal "ra". ss.
     apply (pw_lookup_wf _ u) in WF. ss.
     unfold URA.add in WF. unseal "ra". ss.
@@ -499,23 +557,23 @@ Section WSATS.
     ss. des_ifs.
   Qed. *)
 
-  Lemma wsats_OwnI_open u b n i p (LE : n < b) :
-    OwnI u n i p ∗ wsats u b ∗ OwnE u {[i]} ⊢ |==> ⟦p⟧ ∗ wsats u b ∗ OwnD u {[i]}.
+  (* Lemma wsats_ownI_open u b n i p (LE : n < b) :
+    ownI u n i p ∗ wsats u b ∗ ownE u {[i]} ⊢ |==> ⟦p⟧ ∗ wsats u b ∗ ownD u {[i]}.
   Proof.
     iIntros "(I & SAT & EN)".
     rewrite -(wsats_split u (S n)); last by lia.
     rewrite ?wsats_fold; iDestruct "SAT" as "((SAT1 & SAT2) & SAT3)".
-    iMod (wsat_OwnI_open with "[I SAT1 EN]") as "[P [WSAT D]]"; first iFrame.
+    iMod (wsat_ownI_open with "[I SAT1 EN]") as "[P [WSAT D]]"; first iFrame.
     iModIntro; iFrame.
   Qed.
 
-  Lemma wsats_OwnI_close u b n i p (LE : n < b) :
-    OwnI u n i p -∗ wsats u b -∗ ⟦p⟧ -∗ OwnD u {[i]} ==∗ wsats u b ∗ OwnE u {[i]}.
+  Lemma wsats_ownI_close u b n i p (LE : n < b) :
+    ownI u n i p -∗ wsats u b -∗ ⟦p⟧ -∗ ownD u {[i]} ==∗ wsats u b ∗ ownE u {[i]}.
   Proof.
     iIntros "#I SAT P D".
     rewrite -(wsats_split u (S n)); last by lia.
     rewrite ?wsats_fold; iDestruct "SAT" as "((SAT1 & SAT2) & SAT3)".
-    iMod (wsat_OwnI_close with "[I SAT1 D P]") as "[WSAT EN]"; first by iFrame; done.
+    iMod (wsat_ownI_close with "[I SAT1 D P]") as "[WSAT EN]"; first by iFrame; done.
     iModIntro; iFrame.
   Qed.
 
@@ -525,17 +583,17 @@ Section WSATS.
     unfold closed_universe, used_worlds. iIntros "((W & E & D & FU) & FW)". inv LE; iFrame.
     rewrite (free_worlds_alloc _ b (S m)); [|nia].
     iDestruct "FW" as "[FW L]". iCombine "W L" as "W". rewrite wsats_split; [iFrame|nia].
-  Qed.
+  Qed. *)
 
   (* Lemma empty_worlds_split eu:
-    empty_universes eu ⊢ free_worlds eu 0 ∗ wsats eu 0 ∗ OwnE eu ⊤ ∗ OwnD_auth eu ∗ empty_universes (pos_ext_0 eu) ∗ empty_universes (pos_ext_1 eu).
+    empty_universes eu ⊢ wsat_auth eu 0 ∗ wsats eu 0 ∗ ownE eu ⊤ ∗ ownD_auth eu ∗ empty_universes (pos_ext_0 eu) ∗ empty_universes (pos_ext_1 eu).
   Proof.
     assert (ERA : URA.extends
-              ((OwnER eu ⊤) ⋅
+              ((ownER eu ⊤) ⋅
                (empty_universesR (pos_ext_0 eu) (fun _ => Some ⊤ : CoPset.t)) ⋅
                (empty_universesR (pos_ext_1 eu) (fun _ => Some ⊤ : CoPset.t)))
-              (empty_universesR eu (fun _ => Some ⊤ : CoPset.t) : OwnERA)).
-    { unfold empty_universesR, OwnER, maps_to_res.
+              (empty_universesR eu (fun _ => Some ⊤ : CoPset.t) : ownERA)).
+    { unfold empty_universesR, ownER, maps_to_res.
       exists ε. ur. extensionalities k.
       destruct (excluded_middle_informative _).
       { subst.
@@ -556,11 +614,11 @@ Section WSATS.
     }
 
     assert (DRA : URA.extends
-              ((OwnD_authR eu ∅) ⋅
-               (empty_universesR (pos_ext_0 eu) (fun _ => Auth.black (Some ∅ : Gset.t)) : OwnDRA) ⋅
-               (empty_universesR (pos_ext_1 eu) (fun _ => Auth.black (Some ∅ : Gset.t)) : OwnDRA))
-              (empty_universesR eu (fun _ => Auth.black (Some ∅ : Gset.t)) : OwnDRA)).
-    { unfold empty_universesR, OwnD_authR, maps_to_res.
+              ((ownD_authR eu ∅) ⋅
+               (empty_universesR (pos_ext_0 eu) (fun _ => Auth.black (Some ∅ : Gset.t)) : ownDRA) ⋅
+               (empty_universesR (pos_ext_1 eu) (fun _ => Auth.black (Some ∅ : Gset.t)) : ownDRA))
+              (empty_universesR eu (fun _ => Auth.black (Some ∅ : Gset.t)) : ownDRA)).
+    { unfold empty_universesR, ownD_authR, maps_to_res.
       exists ε. ur. extensionalities k.
       destruct (excluded_middle_informative _).
       { subst.
@@ -580,11 +638,11 @@ Section WSATS.
     }
 
     assert (IRA : URA.extends
-              ((free_worldsR eu 0) ⋅
-               (empty_universesR (pos_ext_0 eu) (fun _ => (fun n => @Auth.black (_ ==> URA.agree (SRFSyn.t n))%ra (fun _ => None)) : URA.pointwise_dep _) : OwnIRA) ⋅
-               (empty_universesR (pos_ext_1 eu) (fun _ => (fun n => @Auth.black (_ ==> URA.agree (SRFSyn.t n))%ra (fun _ => None)) : URA.pointwise_dep _) : OwnIRA))
-              (empty_universesR eu (fun _ => (fun n => @Auth.black (_ ==> URA.agree (SRFSyn.t n))%ra (fun _ => None)) : URA.pointwise_dep _) : OwnIRA)).
-    { unfold empty_universesR, free_worldsR.
+              ((wsat_authR eu 0) ⋅
+               (empty_universesR (pos_ext_0 eu) (fun _ => (fun n => @Auth.black (_ ==> URA.agree (SRFSyn.t n))%ra (fun _ => None)) : URA.pointwise_dep _) : ownIRA) ⋅
+               (empty_universesR (pos_ext_1 eu) (fun _ => (fun n => @Auth.black (_ ==> URA.agree (SRFSyn.t n))%ra (fun _ => None)) : URA.pointwise_dep _) : ownIRA))
+              (empty_universesR eu (fun _ => (fun n => @Auth.black (_ ==> URA.agree (SRFSyn.t n))%ra (fun _ => None)) : URA.pointwise_dep _) : ownIRA)).
+    { unfold empty_universesR, wsat_authR.
       exists ε. ur. ur. extensionalities k n.
       destruct (k =? eu)%positive eqn : EQ.
       { apply Pos.eqb_eq in EQ. subst.
@@ -603,9 +661,9 @@ Section WSATS.
     }
 
     iIntros "(ERA & DRA & IRA)".
-    iPoseProof ((OwnM_extends ERA) with "ERA") as "[[NE E1] E2]".
-    iPoseProof ((OwnM_extends DRA) with "DRA") as "[[ND D1] D2]".
-    iPoseProof ((OwnM_extends IRA) with "IRA") as "[[NI I1] I2]".
+    iPoseProof ((ownM_extends ERA) with "ERA") as "[[NE E1] E2]".
+    iPoseProof ((ownM_extends DRA) with "DRA") as "[[ND D1] D2]".
+    iPoseProof ((ownM_extends IRA) with "IRA") as "[[NI I1] I2]".
     unfold wsats. s. iFrame.
     iExists ∅. eauto.
   Qed.
@@ -630,17 +688,17 @@ Section WSATS.
   Qed. *)
 
 End WSATS.
-
+(* 
 Section FANCY_UPDATE.
 
-  Context `{_W : CtxSL.t}.
-  Context `{_W0 : @GRA.inG OwnIRA Σ}.
-  Context `{_W1 : @GRA.inG OwnERA Γ}.
-  Context `{_W2 : @GRA.inG OwnDRA Γ}.
+  Context `{!CtxSL.t Σ Γ α β τ}.
+  Context `{_W0 : @GRA.inG ownIRA Σ}.
+  Context `{_W1 : @GRA.inG ownERA Γ}.
+  Context `{_W2 : @GRA.inG ownDRA Γ}.
   Notation iProp := (iProp Σ).
 
   Definition inv u (n : level) (N : namespace) p :=
-    (∃ i, ⌜i ∈ (↑N : coPset)⌝ ∧ OwnI u n i p)%I.
+    (∃ i, ⌜i ∈ (↑N : coPset)⌝ ∧ ownI u n i p)%I.
 
   Definition FUpd u b (A : iProp) (E1 E2 : coPset) (P : iProp) : iProp :=
     A ∗ used_worlds u b E1 ==∗ (A ∗ used_worlds u b E2 ∗ P).
@@ -658,18 +716,18 @@ Section FANCY_UPDATE.
     FUpd u b A E1 E2 P ⊢ FUpd u b A (E1 ∪ E) (E2 ∪ E) P.
   Proof.
     iIntros "FUPD (A & WSAT & E & D & U)".
-    iPoseProof (OwnE_disjoint _ _ _ DISJ with "E") as "(E1 & E)".
+    iPoseProof (ownE_disjoint _ _ _ DISJ with "E") as "(E1 & E)".
     iPoseProof ("FUPD" with "[A WSAT E1 D U]") as ">(A & (WSAT & E1 & D & U) & P)"; iFrame.
-    iPoseProof (OwnE_union with "[E E1]") as "EN"; iFrame.
+    iPoseProof (ownE_union with "[E E1]") as "EN"; iFrame.
     iModIntro; eauto.
   Qed.
 
   (* Lemma wsats_inv_gen u b E N n p :
     n < b ->
-    wsats u b ∗ OwnE u E ∗ OwnD_auth u -∗ |==> inv u n N p ∗ (⟦p⟧ -∗ wsats u b) ∗ OwnE u E ∗ OwnD_auth u.
+    wsats u b ∗ ownE u E ∗ ownD_auth u -∗ |==> inv u n N p ∗ (⟦p⟧ -∗ wsats u b) ∗ ownE u E ∗ ownD_auth u.
   Proof.
     iIntros (LT) "(WSAT & EN & DA)".
-    iMod (wsats_OwnI_alloc_lt_gen _ _ _ LT p (fun i => i ∈ ↑N) with "[WSAT DA]") as "(I & D & WSAT)".
+    iMod (wsats_ownI_alloc_lt_gen _ _ _ LT p (fun i => i ∈ ↑N) with "[WSAT DA]") as "(I & D & WSAT)".
     - i. des_ifs. apply iris.base_logic.lib.invariants.fresh_inv_name.
     - iFrame.
     - iModIntro. iFrame.
@@ -695,16 +753,16 @@ Section FANCY_UPDATE.
   Proof.
     iIntros "[% (%iN & #HI)] (A & WSAT & EN & D & R)".
     rewrite {1}(union_difference_L (↑N) E); eauto.
-    iPoseProof (OwnE_disjoint with "EN") as "[EN EE]"; first by set_solver.
+    iPoseProof (ownE_disjoint with "EN") as "[EN EE]"; first by set_solver.
     rewrite {1}(union_difference_singleton_L i (↑N)); eauto.
-    iPoseProof (OwnE_disjoint with "EN") as "[EN Ei]"; first by set_solver.
-    iMod (wsats_OwnI_open u b n i p with "[WSAT EN]") as "(P & SAT & Di)"; [eauto|iFrame; done|].
+    iPoseProof (ownE_disjoint with "EN") as "[EN Ei]"; first by set_solver.
+    iMod (wsats_ownI_open u b n i p with "[WSAT EN]") as "(P & SAT & Di)"; [eauto|iFrame; done|].
     iModIntro; iFrame. iIntros "P [A [WSAT [E [D UNIV]]]]".
-    iMod (wsats_OwnI_close u b n i p with "HI WSAT P Di") as "[SAT EE]"; first by auto.
+    iMod (wsats_ownI_close u b n i p with "HI WSAT P Di") as "[SAT EE]"; first by auto.
     iModIntro; iFrame.
-    iPoseProof (OwnE_union with "[Ei EE]") as "EE"; iFrame.
+    iPoseProof (ownE_union with "[Ei EE]") as "EE"; iFrame.
     rewrite -union_difference_singleton_L; last by eauto.
-    iPoseProof (OwnE_union with "[-]") as "E"; iFrame.
+    iPoseProof (ownE_union with "[-]") as "E"; iFrame.
     rewrite -union_difference_L; by done.
   Qed.
 
@@ -722,10 +780,10 @@ Section FANCY_UPDATE.
     rewrite /FUpd. iIntros (HE) "H (A & WSAT & ENS & D & R)".
     iPoseProof ("H" with "[A WSAT ENS D R]") as ">(A & (WSAT & ENS & D & R) & P)". iFrame.
     iModIntro. rewrite (union_difference_L _ _ HE).
-    iPoseProof (OwnE_disjoint with "ENS") as "(ENS & EN)".
+    iPoseProof (ownE_disjoint with "ENS") as "(ENS & EN)".
     { set_solver. }
     iFrame. iIntros "(A & WSAT & ENS & D & R)". iModIntro. iFrame.
-    iApply OwnE_union. iFrame.
+    iApply ownE_union. iFrame.
   Qed.
 
 
@@ -771,34 +829,34 @@ Section FANCY_UPDATE.
     - iFrame; eauto.
   Qed. *)
 
-  Global Instance from_modal_FUpd u b A E P :
+  (* Global Instance from_modal_FUpd u b A E P :
     FromModal True modality_id (FUpd u b A E E P) (FUpd u b A E E P) P.
   Proof.
     rewrite /FromModal /= /FUpd. iIntros. iModIntro. iFrame. iFrame.
-  Qed.
+  Qed. *)
 
-  Global Instance from_modal_FUpd_general u b A E1 E2 P :
+  (* Global Instance from_modal_FUpd_general u b A E1 E2 P :
     FromModal (E2 ⊆ E1) modality_id P (FUpd u b A E1 E2 P) P.
   Proof.
     rewrite /FromModal /FUpd. ss.
     iIntros (HE) "P (A & WSAT & EN & D & R)". iModIntro. iFrame.
-    iPoseProof ((OwnE_subset _ _ _ HE) with "EN") as "(EN1 & _)". eauto.
+    iPoseProof ((ownE_subset _ _ _ HE) with "EN") as "(EN1 & _)". eauto.
   Qed.
 
   Global Instance from_modal_FUpd_wrong_mask u b A E1 E2 P :
     FromModal (pm_error "Only non-mask-changing update modalities can be introduced directly.
-Use [FUpd_mask_frame] and [FUpd_intro_mask]")
+  Use [FUpd_mask_frame] and [FUpd_intro_mask]")
               modality_id (FUpd u b A E1 E2 P) (FUpd u b A E1 E2 P) P | 100.
   Proof.
     intros [].
-  Qed.
+  Qed. *)
 
-  Global Instance elim_modal_bupd_FUpd p u b A E1 E2 P Q :
+  (* Global Instance elim_modal_bupd_FUpd p u b A E1 E2 P Q :
     ElimModal True p false (|==> P) P (FUpd u b A E1 E2 Q) (FUpd u b A E1 E2 Q) | 10.
   Proof.
     rewrite /ElimModal bi.intuitionistically_if_elim /FUpd.
     iIntros (_) "(>P & K) I". iApply ("K" with "P"). iFrame.
-  Qed.
+  Qed. *)
 
   Global Instance elim_modal_FUpd_FUpd u p b b' A E1 E2 E3 P Q :
     ElimModal (b <= b') p false (FUpd u b A E1 E2 P) P (FUpd u b' A E1 E3 Q) (FUpd u b' A E2 E3 Q).
@@ -874,7 +932,7 @@ Use [FUpd_mask_frame] and [FUpd_intro_mask]")
 
 End FANCY_UPDATE.
 
-Global Opaque FUpd.
+Global Opaque FUpd. *)
 
 (* Goal (nroot .@ "gil") ## (nroot .@ "hur"). *)
 (* eauto with solve_ndisj. *)
