iris_system/iprop.v
@@ -7,9 +7,9 @@ From iris.algebra Require Import cmra updates functions gmap_view.
 From CRIS.base_logic Require Export base_logic.
 From CRIS.lib Require Import allocs.
 
-(** * Discrete unital resource algebras (internal use only) *)
+(** * Discrete resource algebras (internal use only) *)
 Record DRA := DRA_mk {
-  DRA_RA :> ucmra;
+  DRA_RA :> cmra;
   DRA_discrete : CmraDiscrete DRA_RA
 }.
 Global Arguments DRA_mk _ {_}.
@@ -31,8 +31,8 @@ Global Coercion GRAUR : GRA >-> ucmra.
 Global Instance GRA_discrete {Σ : GRA} : CmraDiscrete Σ.
 Proof. apply _. Qed.
 
-(** * Typeclass for individual ucmras being included in GRAs *)
-Class inG (RA : ucmra) (Σ : GRA) := inG_mk {
+(** * Typeclass for individual cmras being included in GRAs *)
+Class inG (RA : cmra) (Σ : GRA) := inG_mk {
   inG_id : gid Σ;
   inG_prf : RA = GRA_lookup Σ inG_id
 }.
@@ -42,19 +42,22 @@ Global Hint Mode inG ! - : typeclass_instances.
 Module GRAs.
   Definition nil : GRA := GRA_mk 0 (fin_0_inv _).
 
-  Definition singleton (RA : ucmra) `{CmraDiscrete RA} : GRA :=
-    GRA_mk 1 (fin_S_inv (λ _, DRA) (DRA_mk RA) (fin_0_inv _)).
+  Definition singleton (A : DRA) : GRA :=
+    GRA_mk 1 (fin_S_inv (λ _, DRA) A (fin_0_inv _)).
 
   Program Definition app (Σ1 Σ2 : GRA) : GRA :=
     GRA_mk (GRA_len Σ1 + GRA_len Σ2) (fin_add_inv _ (GRA_lookup Σ1) (GRA_lookup Σ2)).
 End GRAs.
+Global Coercion GRAs.singleton : DRA >-> GRA.
 Notation "#[ ]" := GRAs.nil (format "#[ ]").
+(* TODO : Reversible coercions do not work - find a way *)
+Notation "[ R ]" := (DRA_mk R).
 Notation "#[ Σ1 ; .. ; Σn ]" := (GRAs.app Σ1 .. (GRAs.app Σn GRAs.nil) ..).
+(* Notation "#[ Σ1  .. ; Σn ]" := (GRAs.app (DRA_mk Σ1) .. (GRAs.app (DRA_mk Σn) GRAs.nil) ..). *)
 
 (** * GRA being included in another GRA *)
-Class subG (Σ1 Σ2 : GRA) := in_subG i :
+Class subG (Σ1 Σ2 : GRA) := subG_in i :
   { j | GRA_lookup Σ1 i = GRA_lookup Σ2 j }.
-
 Global Hint Mode subG ! + : typeclass_instances.
 
 Lemma subG_inv Σ1 Σ2 Σ : subG (GRAs.app Σ1 Σ2) Σ → subG Σ1 Σ * subG Σ2 Σ.
@@ -76,99 +79,50 @@ Proof.
   move=> H i; move: H=> /(_ i) [j ?].
   exists (Fin.R _ j). by rewrite /= fin_add_inv_r.
 Qed.
+Global Instance index_inG Σ (i : gid Σ) : inG (GRA_lookup Σ i) Σ.
+Proof.
+  econstructor; eauto.
+Defined.
+Global Program Instance in_subG Σ1 Σ2 `{M : cmra} `{emb : inG M Σ1} : subG Σ1 Σ2 → inG M Σ2.
+Next Obligation.
+  intros. destruct emb. destruct (s inG_id0). exact x.
+Defined.
+Next Obligation.
+  intros. destruct emb. simpl. destruct (s inG_id0). subst. f_equal. eauto.
+Defined.
+Lemma subG_inG Σ (A : DRA) : subG A Σ → inG A Σ.
+Proof.
+  intros H; destruct (H 0%fin). exists x. rewrite -e. econstructor.
+Qed.
+(** This tactic solves the usual obligations "subG ? Σ → {in,?}G ? Σ" *)
+Ltac solve_inG :=
+  (* Get all assumptions *)
+  intros;
+  (* Unfold the top-level xΣ. We need to support this to be a function. *)
+  lazymatch goal with
+  | H : subG (?xΣ _ _ _ _) _ |- _ => try unfold xΣ in H
+  | H : subG (?xΣ _ _ _) _ |- _ => try unfold xΣ in H
+  | H : subG (?xΣ _ _) _ |- _ => try unfold xΣ in H
+  | H : subG (?xΣ _) _ |- _ => try unfold xΣ in H
+  | H : subG ?xΣ _ |- _ => try unfold xΣ in H
+  end;
+  (* Take apart subG for non-"atomic" lists *)
+  repeat match goal with
+         | H : subG (GRAs.app _ _) _ |- _ => apply subG_inv in H; destruct H
+         end;
+  (* Try to turn singleton subG into inG; but also keep the subG for typeclass
+     resolution -- to keep them, we put them onto the goal. *)
+  repeat match goal with
+         | H : subG _ _ |- _ => move:(H); (apply subG_inG in H || clear H)
+         end;
+  (* Again get all assumptions and simplify the functors *)
+  intros; simpl in *;
+  (* We support two kinds of goals: Things convertible to inG;
+     and records with inG and typeclass fields. Try to solve the
+     first case. *)
+  try assumption;
+  (* That didn't work, now we're in for the second case. *)
+  split; (assumption || by apply _).
 
 (* iProps are parameterized on GRAs, without step-indexing *)
-Section iProp.
-  Context {Σ : GRA}.
-  Definition iProp := uPredI Σ.
-End iProp.
-Global Arguments iProp {_}.
-
-
-  (* Program Definition of_list (RAs : ucmra_list) : t :=
-    {| gra_map := λ n, (UList.nth n RAs (optionUR Empty_setR)) |}.
-  Next Obligation. induction RAs; destruct i; apply _. Qed.
-
-  Definition to_URA (Σ : t) : ucmra := discrete_funUR Σ.
-  Coercion to_URA : t >-> ucmra.
-
-
-
-  Global Instance inG_cmra_discrete `{!inG A Σ} : CmraDiscrete A.
-  Proof. erewrite inG_prf. apply _. Qed.
-
-  (* a : cmra_car =ty= RAs inG_id =ty= RAs n *)
-  Definition embed `{!inG A Σ} (a : A) : Σ :=
-    discrete_fun_singleton inG_id (cmra_transport (f_equal _ inG_prf) a).
-  Local Instance : Params (@embed) 3 := {}. *)
-
-(* Section lemmas.
-  Context `{!inG A Σ}.
-  Implicit Types a : A.
-
-  Lemma embed_wf
-        a
-        (WF : ✓ embed a)
-    :
-      <<WF : ✓ a>>
-  .
-  Proof. by rewrite /embed discrete_fun_singleton_valid cmra_transport_valid in WF. Qed.
-
-  Lemma wf_embed
-        a
-        (WF : ✓ a)
-    :
-      <<WF : ✓ embed a >>
-  .
-  Proof. by rewrite /NW /embed discrete_fun_singleton_valid cmra_transport_valid. Qed.
-
-  Global Instance embed_ne : NonExpansive (@embed A Σ _).
-  Proof. by intros ????; apply discrete_fun_singleton_ne, cmra_transport_ne. Qed.
-  Global Instance embed_proper : Proper ((≡) ==> (≡)) (@embed A Σ _) := ne_proper _.
-
-  Lemma embed_add
-        a0 a1
-    :
-      embed a0 ⋅ embed a1 ≡ embed (a0 ⋅ a1)
-    .
-  Proof. by rewrite /embed discrete_fun_singleton_op cmra_transport_op. Qed.
-
-  Lemma embed_updatable_set
-        a P
-        (UPD : a ~~>: P)
-    :
-      <<UPD : embed a ~~>: λ b, ∃ a', b = embed a' ∧ P a' >>
-  .
-  Proof.
-    eapply discrete_fun_singleton_updateP.
-    { eapply cmra_transport_updateP', UPD. }
-    ii. ss. des. subst. eauto.
-  Qed.
-
-  Lemma embed_updatable
-        a0 a1
-        (UPD : a0 ~~> a1)
-    :
-      <<UPD : embed a0 ~~> embed a1 >>
-  .
-  Proof.
-    eapply cmra_update_updateP, cmra_updateP_weaken.
-    - apply embed_updatable_set, cmra_update_updateP, UPD.
-    - ii. ss. des. subst. done.
-  Qed.
-
-  Lemma embed_core a : embed (core a) ≡ core (embed a).
-  Proof. by rewrite /embed discrete_fun_singleton_core cmra_transport_core. Qed.
-
-  (* Note : NOT a general lemma for [cmra_transport]. Tailed for the proof pattern
-    of [GRA]. I.e., upstreaming this to iris doesn't make sense. *)
-  Local Lemma cmra_transport_unit {B C : ucmra} (H : B = C) : cmra_transport (f_equal _ H) ε = ε.
-  Proof. by destruct H. Qed.
-  Lemma embed_unit : embed ε ≡ ε.
-  Proof. by rewrite /embed cmra_transport_unit discrete_fun_singleton_unit. Qed.
-
-End lemmas.
-End GRA.
-Coercion GRA.to_URA : GRA.t >-> ucmra.
-
-Global Opaque GRA.to_URA. *)
+Notation iProp Σ := (uPredI Σ).
