iris_system/own.v
@@ -1,7 +1,8 @@
-From iris.algebra Require Import proofmode_classes functions.
+From iris.algebra Require Import proofmode_classes functions coPset.
 From iris.proofmode Require Export proofmode.
 From CRIS.base_logic Require Export base_logic.
 From CRIS.lib Require Import allocs.
+Require Import sflib.
 Require Import Level.
 Require Export iprop.
 Import uPred.
@@ -25,74 +26,73 @@ End uPredI.
 (* uPredI_affine is added so that IPM can also resolve pure predicates with evars. *)
 Global Hint Immediate uPredI_affine : core. *)
 
-(* TODO : 1) refactor GRA.t
-          2) move iProp and own to a separate file *)
-Local Definition iRes_singleton `{i : inG A Σ} (γ : gname) (a : A) : Σ :=
-  discrete_fun_singleton (inG_id i) (allocs_frag γ (cmra_transport (f_equal _  inG_prf) a)).
+(* TODO : 1) refactor GRA
+          2) move iProp Σ and own to a separate file *)
+Local Definition iRes_singleton `{i : !inG A Σ} (γ : gname) (a : A) : Σ :=
+  discrete_fun_singleton (inG_id i) (allocs_frag γ (cmra_transport inG_prf a)).
 Global Instance: Params (@iRes_singleton) 4 := {}.
 
 (** * Definitions of resource ownership with ghost locations. *)
-Local Definition own_def `{!inG A Σ} (γ : gname) (a : A) : iProp := uPred_ownM (iRes_singleton γ a).
+Local Definition own_def `{!inG A Σ} (γ : gname) (a : A) : iProp Σ :=
+  uPred_ownM (iRes_singleton γ a).
 Local Definition own_aux : seal (@own_def). Proof. by eexists. Qed.
 Definition own := own_aux.(unseal).
 Local Definition own_eq : @own = @own_def := own_aux.(seal_eq).
 Global Arguments own {_ _ _} γ a.
 
-Local Program Definition own_admin_def Σ {υ : mod_level} : iProp :=
-  ∃ (a : positive), uPred_ownM
-    ((λ i, @allocs_auth (GRA_lookup Σ i)
-      (λ b, (∃ c, b = 2 ^ υ * 3 ^ c ∧ a <= c)%positive)%type _) : GRAUR Σ).
-Next Obligation.
+(* TODO : Think later if mod_levels can be erased *)
+Local Program Definition own_admin_def (Σ : GRA) : iProp Σ :=
+  ∃ (X : coPset), ⌜set_infinite X⌝
+    ∗ uPred_ownM ((λ i, @allocs_auth (GRA_lookup Σ i) X) : GRAUR Σ).
 Local Definition own_admin_aux : seal (@own_admin_def). Proof. by eexists. Qed.
 Definition own_admin := own_admin_aux.(unseal).
 Local Definition own_admin_eq : @own_admin = @own_admin_def := own_admin_aux.(seal_eq).
-Global Arguments own_admin {_ _}.
+Global Arguments own_admin {_}.
 
-(** * Definitions of resource ownership - for metatheoretical results only *)
-Local Definition Own_def {Σ : GRA} (a : Σ) : iProp := uPred_ownM a.
+(** * Definitions of resource ownership - for metatheoretical uses only *)
+Local Definition Own_def {Σ : GRA} (a : Σ) : iProp Σ := uPred_ownM a.
 Local Definition Own_aux : seal (@Own_def). Proof. by eexists. Qed.
 Definition Own := Own_aux.(unseal).
 Local Definition Own_eq : @Own = @Own_def := Own_aux.(seal_eq).
 Global Arguments Own {Σ} a.
 
 Section properties.
-  Context `{i : !inG A Σ} {υ : mod_level}.
+  Context `{i : !inG A Σ}.
   Implicit Types a : A.
 
-  Local Instance iRes_singleton_ne γ : NonExpansive (@iRes_singleton A Σ _ υ γ).
+  Local Instance iRes_singleton_ne γ : NonExpansive (@iRes_singleton A Σ _ γ).
   Proof.
-    by intros ????;
-      apply discrete_fun_singleton_ne, singleton_ne, allocs_frag_ne, cmra_transport_ne.
+    by intros ????; apply discrete_fun_singleton_ne, allocs_frag_ne, cmra_transport_ne.
   Qed.
   Local Instance iRes_singleton_proper γ :
-    Proper ((≡) ==> (≡)) (@iRes_singleton A Σ _ υ γ) := ne_proper _.
+    Proper ((≡) ==> (≡)) (@iRes_singleton A Σ _ γ) := ne_proper _.
   Local Lemma iRes_singleton_op γ a1 a2 :
     iRes_singleton γ (a1 ⋅ a2) ≡ iRes_singleton γ a1 ⋅ iRes_singleton γ a2.
   Proof.
-    rewrite /iRes_singleton discrete_fun_singleton_op singleton_op cmra_transport_op.
-    f_equiv. apply: singletonM_proper; rewrite allocs_frag_op; done.
+    rewrite /iRes_singleton discrete_fun_singleton_op cmra_transport_op.
+    f_equiv. rewrite allocs_frag_op; done.
   Qed.
   Local Lemma iRes_singleton_validI γ a : ✓ (iRes_singleton γ a) ⊢@{@iProp Σ} ✓ a.
   Proof.
     rewrite /iRes_singleton /allocs_frag.
     rewrite discrete_fun_validI (forall_elim (inG_id i)) discrete_fun_lookup_singleton.
-    rewrite singleton_validI discrete_fun_validI (forall_elim γ) discrete_fun_lookup_singleton.
+    rewrite discrete_fun_validI (forall_elim γ) discrete_fun_lookup_singleton.
     rewrite option_validI csum_validI.
-    trans (✓ cmra_transport (f_equal _ inG_prf) a : @iProp Σ)%I; last by destruct inG_prf.
+    trans (✓ cmra_transport inG_prf a : @iProp Σ)%I; last by destruct inG_prf.
     done.
   Qed.
 
   (** ** Properties of [own] *)
-  Global Instance own_ne γ : NonExpansive (@own A Σ _ υ γ).
+  Global Instance own_ne γ : NonExpansive (@own A Σ _ γ).
   Proof. rewrite !own_eq; solve_proper. Qed.
-  Global Instance own_proper γ : Proper ((≡) ==> (⊣⊢)) (@own A Σ _ υ γ) := ne_proper _.
+  Global Instance own_proper γ : Proper ((≡) ==> (⊣⊢)) (@own A Σ _ γ) := ne_proper _.
 
   Lemma own_op γ a1 a2 : own γ (a1 ⋅ a2) ⊣⊢ own γ a1 ∗ own γ a2.
   Proof. by rewrite !own_eq -ownM_op -iRes_singleton_op. Qed.
   Lemma own_mono γ a1 a2 : a2 ≼ a1 → own γ a1 ⊢ own γ a2.
   Proof. move=> [c ->]. by rewrite own_op sep_elim_l. Qed.
 
-  Global Instance own_mono' γ : Proper (flip (≼) ==> (⊢)) (@own A Σ _ υ γ).
+  Global Instance own_mono' γ : Proper (flip (≼) ==> (⊢)) (@own A Σ _ γ).
   Proof. intros a1 a2. apply own_mono. Qed.
 
   Lemma own_valid γ a : own γ a ⊢ ✓ a.
@@ -111,116 +111,80 @@ Section properties.
   Global Instance own_core_persistent γ a : CoreId a → Persistent (own γ a).
   Proof. rewrite !own_eq /own_def; apply _. Qed.
 
-  (* Lemma own_alloc a : ✓ a → own_gen A ⊢ |==> own_gen A ∗ ∃ γ, own γ a. *)
-  (* Proof. *)
-    (* intros Ha. *)
-    (* rewrite -(bupd_mono (∃ m, ⌜∃ γ, m = iRes_singleton γ a⌝ ∧ uPred_ownM m ∗ own_gen A)%I). *)
-    (* { rewrite own_gen_eq. apply bupd_ownM_update. }   *)
-    (* ; iIntros "GEN". eapply (own_alloc_dep (λ _, a)); eauto. Qed. *)
-(* TODO : Stuck here *)
-(** ** Allocation *)
-(* Lemma own_alloc_strong_dep (f : gname → A) (P : gname → Prop) :
-  pred_infinite P →
-  (∀ γ, P γ → ✓ (f γ)) →
-  ⊢ |==> ∃ γ, ⌜P γ⌝ ∗ own γ (f γ).
-Proof.
-  intros HPinf Hf.
-  rewrite -(bupd_mono (∃ m, ⌜∃ γ, P γ ∧ m = iRes_singleton γ (f γ)⌝ ∧ uPred_ownM m)%I).
-  - rewrite /bi_emp_valid (ownM_unit emp).
-    apply bupd_ownM_updateP, (discrete_fun_singleton_updateP_empty _ (λ m, ∃ γ,
-      m = {[ γ := inG_unfold (cmra_transport inG_prf (f γ)) ]} ∧ P γ));
-      [|naive_solver].
-    apply (alloc_updateP_strong_dep _ P _ (λ γ,
-      inG_unfold (cmra_transport inG_prf (f γ)))); [done| |naive_solver].
-    intros γ _ ?.
-    by apply (cmra_morphism_valid inG_unfold), cmra_transport_valid, Hf.
-  - apply exist_elim=>m; apply pure_elim_l=>-[γ [Hfresh ->]].
-    by rewrite !own_eq /own_def -(exist_intro γ) pure_True // left_id.
-Qed.
-Lemma own_alloc_cofinite_dep (f : gname → A) (G : gset gname) :
-  (∀ γ, γ ∉ G → ✓ (f γ)) → ⊢ |==> ∃ γ, ⌜γ ∉ G⌝ ∗ own γ (f γ).
-Proof.
-  intros Ha.
-  apply (own_alloc_strong_dep f (λ γ, γ ∉ G))=> //.
-  apply (pred_infinite_set (C:=gset gname)).
-  intros E. set (γ := fresh (G ∪ E)).
-  exists γ. apply not_elem_of_union, is_fresh.
-Qed.
-Lemma own_alloc_dep (f : gname → A) :
-  (∀ γ, ✓ (f γ)) → ⊢ |==> ∃ γ, own γ (f γ).
-Proof.
-  intros Ha. rewrite /bi_emp_valid (own_alloc_cofinite_dep f ∅) //; [].
-  apply bupd_mono, exist_mono=>?. apply: sep_elim_r.
-Qed.
+  (* TODO : Find a way to hide own_admin using fancy-update-like modalities *)
+  (* Note : There is no way to impose restrictions on ghost locs for now. *)
+  Lemma own_alloc a : ✓ a → own_admin ⊢ |==> own_admin ∗ ∃ γ, own γ a.
+  Proof.
+    intros hwf. rewrite ?own_admin_eq /own_admin_def.
+    iIntros "[%X [%INF OWN]]".
+    iPoseProof (bupd_ownM_update _
+      (((λ i, allocs_auth (GRA_lookup Σ i) (X ∖ {[coPpick X]})) : GRAUR Σ)
+      ⋅ iRes_singleton (coPpick X) a)
+      with "OWN") as "> [AUTH OWN]".
+    { apply discrete_fun_update; intros i'; destruct (decide ((inG_id i) = i')).
+      { subst i'.
+        rewrite discrete_fun_lookup_op. etrans.
+        { eapply (allocs_alloc (cmra_transport inG_prf a) X (coPpick X)).
+          { eapply coPpick_elem_of, coPset_infinite_finite; eauto. }
+          { apply cmra_transport_valid. apply hwf. }
+        }
+        apply cmra_update_op.
+        { done. }
+        { rewrite /iRes_singleton discrete_fun_lookup_singleton; done. }
+      }
+      { rewrite discrete_fun_lookup_op /iRes_singleton discrete_fun_lookup_singleton_ne; eauto.
+        rewrite right_id.
+        etrans.
+        eapply (allocs_auth_split (X ∖ {[coPpick X]}) {[coPpick X]}); try set_solver.
+        { set_unfold; intros x; split; intros H; des; eauto.
+          { destruct (decide (x = coPpick X)); eauto. }
+          { subst; eapply coPpick_elem_of, coPset_infinite_finite; eauto. }
+        }
+        apply cmra_update_op_l.
+      }
+    }
+    iModIntro; iFrame.
+    iSplit; eauto.
+    { iPureIntro. eapply difference_infinite, singleton_finite; eauto. }
+    { iExists (coPpick X); rewrite own_eq /own_def; done. }
+  Qed.
 
-Lemma own_alloc_strong a (P : gname → Prop) :
-  pred_infinite P →
-  ✓ a → ⊢ |==> ∃ γ, ⌜P γ⌝ ∗ own γ a.
-Proof. intros HP Ha. eapply (own_alloc_strong_dep (λ _, a)); eauto. Qed.
-Lemma own_alloc_cofinite a (G : gset gname) :
-  ✓ a → ⊢ |==> ∃ γ, ⌜γ ∉ G⌝ ∗ own γ a.
-Proof. intros Ha. eapply (own_alloc_cofinite_dep (λ _, a)); eauto. Qed.
+  Lemma own_update γ a a' : a ~~> a' → own γ a ⊢ |==> own γ a'.
+  Proof.
+    rewrite ?own_eq /own_def; intros upd.
+    eapply bupd_ownM_update, discrete_fun_singleton_update, allocs_frag_update.
+    destruct inG_prf. eapply cmra_update_updateP, cmra_updateP_weaken; cycle 1.
+    { intros y Hy; eapply Hy. }
+    { eapply cmra_transport_updateP.
+      { eapply cmra_update_updateP, upd. }
+      { intros y <-; eauto. }
+    }
+  Qed.
 
-(** ** Frame preserving updates *)
-Lemma own_updateP P γ a : a ~~>: P → own γ a ⊢ |==> ∃ a', ⌜P a'⌝ ∗ own γ a'.
-Proof.
-  intros Hupd. rewrite !own_eq.
-  rewrite -(bupd_mono (∃ m,
-    ⌜ ∃ a', m = iRes_singleton γ a' ∧ P a' ⌝ ∧ uPred_ownM m)%I).
-  - apply bupd_ownM_updateP, (discrete_fun_singleton_updateP _ (λ m, ∃ x,
-      m = {[ γ := x ]} ∧ ∃ x',
-      x = inG_unfold x' ∧ ∃ a',
-      x' = cmra_transport inG_prf a' ∧ P a')); [|naive_solver].
-    apply singleton_updateP', (iso_cmra_updateP' inG_fold).
-    { apply inG_unfold_fold. }
-    { apply (cmra_morphism_op _). }
-    { apply inG_unfold_validN. }
-    by apply cmra_transport_updateP'.
-  - apply exist_elim=> m; apply pure_elim_l=> -[a' [-> HP]].
-    rewrite -(exist_intro a'). rewrite -persistent_and_sep.
-    by apply and_intro; [apply pure_intro|].
-Qed.
-
-Lemma own_update γ a a' : a ~~> a' → own γ a ⊢ |==> own γ a'.
-Proof.
-  intros. iIntros "?".
-  iMod (own_updateP (a' =.) with "[$]") as (a'') "[-> $]".
-  { by apply cmra_update_updateP. }
-  done.
-Qed.
-Lemma own_update_2 γ a1 a2 a' :
-  a1 ⋅ a2 ~~> a' → own γ a1 -∗ own γ a2 ==∗ own γ a'.
-Proof. intros. apply entails_wand, wand_intro_r. rewrite -own_op. by iApply own_update. Qed.
-Lemma own_update_3 γ a1 a2 a3 a' :
-  a1 ⋅ a2 ⋅ a3 ~~> a' → own γ a1 -∗ own γ a2 -∗ own γ a3 ==∗ own γ a'.
-Proof. intros. apply entails_wand. do 2 apply wand_intro_r. rewrite -!own_op. by iApply own_update. Qed.
-End global.
+  Lemma own_update_2 γ a1 a2 a' :
+    a1 ⋅ a2 ~~> a' → own γ a1 -∗ own γ a2 ==∗ own γ a'.
+  Proof. intros. apply entails_wand, wand_intro_r. rewrite -own_op. by iApply own_update. Qed.
+  Lemma own_update_3 γ a1 a2 a3 a' :
+    a1 ⋅ a2 ⋅ a3 ~~> a' → own γ a1 -∗ own γ a2 -∗ own γ a3 ==∗ own γ a'.
+  Proof.
+    intros. apply entails_wand. do 2 apply wand_intro_r. rewrite -!own_op.
+    by iApply own_update.
+  Qed.
+End properties.
 
 Global Arguments own_valid {_ _} [_] _ _.
 Global Arguments own_valid_2 {_ _} [_] _ _ _.
 Global Arguments own_valid_3 {_ _} [_] _ _ _ _.
 Global Arguments own_valid_l {_ _} [_] _ _.
 Global Arguments own_valid_r {_ _} [_] _ _.
-Global Arguments own_updateP {_ _} [_] _ _ _ _.
 Global Arguments own_update {_ _} [_] _ _ _ _.
 Global Arguments own_update_2 {_ _} [_] _ _ _ _ _.
 Global Arguments own_update_3 {_ _} [_] _ _ _ _ _ _.
 
-Lemma own_unit A `{i : !inG Σ (A:ucmra)} γ : ⊢ |==> own γ (ε:A).
-Proof.
-  rewrite /bi_emp_valid (ownM_unit emp) !own_eq /own_def.
-  apply bupd_ownM_update, discrete_fun_singleton_update_empty.
-  apply (alloc_unit_singleton_update (inG_unfold (cmra_transport inG_prf ε))).
-  - apply (cmra_morphism_valid _), cmra_transport_valid, ucmra_unit_valid.
-  - intros x. rewrite -(inG_unfold_fold x) -(cmra_morphism_op inG_unfold).
-    f_equiv. generalize (inG_fold x)=> x'.
-    destruct inG_prf=> /=. by rewrite left_id.
-  - done.
-Qed.
 
 (** Big op class instances *)
 Section big_op_instances.
-  Context `{!inG Σ (A:ucmra)}.
+  Context `{!inG (A:ucmra) Σ}.
 
   Global Instance own_cmra_sep_homomorphism γ :
     WeakMonoidHomomorphism op uPred_sep (≡) (own γ).
@@ -267,7 +231,7 @@ End big_op_instances.
 
 (** Proofmode class instances *)
 Section proofmode_instances.
-  Context `{!inG Σ A}.
+  Context `{!inG A Σ}.
   Implicit Types a b : A.
 
   Global Instance into_sep_own γ a b1 b2 :
@@ -280,14 +244,12 @@ Section proofmode_instances.
   Global Instance from_sep_own γ a b1 b2 :
     IsOp a b1 b2 → FromSep (own γ a) (own γ b1) (own γ b2).
   Proof. intros. by rewrite /FromSep -own_op -is_op. Qed.
-  (* TODO: Improve this instance with generic own simplification machinery
-  once https://gitlab.mpi-sws.org/iris/iris/-/issues/460 is fixed *)
+
   (* Cost > 50 to give priority to [combine_sep_as_fractional]. *)
   Global Instance combine_sep_as_own γ a b1 b2 :
     IsOp a b1 b2 → CombineSepAs (own γ b1) (own γ b2) (own γ a) | 60.
   Proof. intros. by rewrite /CombineSepAs -own_op -is_op. Qed.
-  (* TODO: Improve this instance with generic own validity simplification
-  machinery once https://gitlab.mpi-sws.org/iris/iris/-/issues/460 is fixed *)
+  
   Global Instance combine_sep_gives_own γ b1 b2 :
     CombineSepGives (own γ b1) (own γ b2) (✓ (b1 ⋅ b2)).
   Proof.
@@ -302,75 +264,41 @@ Section proofmode_instances.
     destruct Hb; by rewrite persistent_and_sep.
   Qed.
 End proofmode_instances.
+(* TODO : Lemma own_unit A `{i : !inG (A:ucmra) Σ} γ : own_admin ⊢ |==> own_admin ∗ own γ (ε:A). *)
 
 
-Section iProp.
-  Local Definition Own_def `{!inG (a : Σ) : iProp := uPred_ownM a.
-  Local Definition Own_aux : seal (@Own_def). Proof. by eexists. Qed.
-  Definition Own := Own_aux.(unseal).
-  Definition Own_eq : @Own = @Own_def := Own_aux.(seal_eq).
+Section Own.
+  Context `{Σ : GRA}.
+  Implicit Types a b : Σ.
+  Notation iProp Σ := (iProp Σ Σ).
 
-  Definition OwnM {M : ucmra} `{!inG M Σ} (γ : gname) (a : M) : iProp := Own (GRA.embed a).
-
-  (* Global Instance iProp_bi_bupd : BiBUpd iProp := uPred_bi_bupd Σ. *)
-
-  Definition from_upred (P : uPred Σ) : iProp := P.
-  Definition to_upred (P : iProp) : uPred Σ := P.
-
-End iProp.
-Global Arguments iProp : clear implicits.
-Arguments OwnM : simpl never.
-
-Local Ltac unseal := rewrite ?Own_eq /Own_def.
-
-Section TEST.
-  Context {Σ : GRA.t}.
-  Notation iProp := (iProp Σ).
-
-  Goal forall (P Q R : iProp) (PQ : P -∗ Q) (QR : Q -∗ R), P -∗ R.
-  Proof.
-    iIntros (P Q R PQ QR) "H".
-    iApply QR. iApply PQ. iApply "H".
-  Qed.
-
-  Goal forall (P Q : iProp), ((|==> P) ∗ Q) -∗ (|==> Q).
-  Proof.
-    i. iStartProof.
-    iIntros "[Hxs Hys]". iMod "Hxs". iApply "Hys".
-  Qed.
-End TEST.
-
-Section class_instances.
-  Context `{Σ : GRA.t}.
-  Notation iProp := (iProp Σ).
+  Local Ltac unseal := rewrite Own_eq /Own_def.
 
   Global Instance Own_ne : NonExpansive (@Own Σ).
   Proof. unseal. solve_proper. Qed.
-  Global Instance Own_proper :
-    Proper ((≡) ==> (⊣⊢)) (@Own Σ) := ne_proper _.
+  Global Instance Own_proper : Proper ((≡) ==> (⊣⊢)) (@Own Σ) := ne_proper _.
 
   Global Instance Own_core_persistent a : CoreId a → Persistent (@Own Σ a).
-  Proof. rewrite !Own_eq /Own_def; apply _. Qed.
+  Proof. unseal; apply _. Qed.
 
-  Lemma Own_Upd r1 r2 (UPD : r1 ~~> r2) :
-    Own r1 ⊢ |==> Own r2.
+  Lemma Own_Upd a b (UPD : a ~~> b) : Own a ⊢ |==> Own b.
   Proof.
     unseal; iIntros "Hr1"; iPoseProof (uPred.bupd_ownM_update with "Hr1") as "Hr2"; eauto.
   Qed.
 
-  Lemma Own_op (a1 a2 : Σ) :
-    (Own (a1 ⋅ a2)) ⊣⊢ (Own a1 ∗ Own a2).
-  Proof. unseal. by rewrite uPred.ownM_op. Qed.
+  Lemma Own_extends (a b : Σ) (EXT : a ≼ b) : Own b ⊢ Own a .
+  Proof. unseal. apply uPred.ownM_mono. done. Qed.
 
-  Lemma Own_valid (a : Σ) :
-    Own a ⊢ ⌜✓ a⌝.
+  Lemma Own_op a b : Own (a ⋅ b) ⊣⊢ Own a ∗ Own b.
+  Proof. by unseal; rewrite uPred.ownM_op. Qed.
+
+  Lemma Own_valid a : Own a ⊢ ⌜✓ a⌝.
   Proof.
     unseal. iIntros "H". iDestruct (uPred.ownM_valid with "H") as "V".
     iEval (rewrite uPred.discrete_valid) in "V". iFrame "V".
   Qed.
 
-  Lemma Own_wand_valid (a1 a2 : Σ) (WAND : Own a1 ⊢ |==> Own a2) (VALID : ✓ a1) :
-    ✓ a2.
+  Lemma Own_wand_valid (a1 a2 : Σ) (WAND : Own a1 ⊢ |==> Own a2) (VALID : ✓ a1) : ✓ a2.
   Proof.
     eapply uPred.bupd_ownM_update_2; last by exact VALID.
     move: WAND; unseal; eauto.
@@ -388,17 +316,17 @@ Section class_instances.
     ∃ a1 a2, a ≡ a1 ⋅ a2 ∧ (Own a1 ⊢ P) ∧ (Own a2 ⊢ Q).
   Proof.
     uPred.unseal_in IMPL; apply IMPL in VALID;
-      last (rewrite IPM.Own_eq /IPM.Own_def; uPred.unseal; exists ε; eauto; rewrite right_id //=).
+      last (unseal; uPred.unseal; exists ε; eauto; rewrite right_id //=).
     destruct VALID as [a1 [a2 [Ha VALID]]]; des; exists a1, a2; split; eauto; split; econs; intros x wfx Own;
-      rewrite IPM.Own_eq /IPM.Own_def in Own; uPred.unseal_in Own; destruct Own as [? ->]; eauto using uPred_mono.
+      rewrite Own_eq /Own_def in Own; uPred.unseal_in Own; destruct Own as [? ->]; eauto using uPred_mono.
   Qed.
 
-  Lemma Own_bupd_update r1 r2 (UPD : Own r1 ⊢ |==> Own r2) :
-    r1 ~~> r2.
+  Lemma Own_bupd_update a b (UPD : Own a ⊢ |==> Own b) :
+    a ~~> b.
   Proof.
-    move: UPD; unseal; uPred.unseal; intros UPD.
+    move: UPD; repeat unseal; uPred.unseal; intros UPD.
     rewrite cmra_discrete_total_update; intros z wf.
-    destruct UPD as [UPD]; exploit (UPD r1); ss.
+    destruct UPD as [UPD]; exploit (UPD a); ss.
     { eauto using cmra_valid_op_l. }
     { exists ε; rewrite right_id //. }
     { intros [x' H]; exploit (H z) => //=.
@@ -407,24 +335,24 @@ Section class_instances.
     }
   Qed.
 
-  Lemma Own_pure_soundness x P (VALID : ✓ x) (DERIV : Own x ⊢ ⌜P⌝) : P.
+  Lemma Own_pure_soundness a P (VALID : ✓ a) (DERIV : Own a ⊢ ⌜P⌝) : P.
   Proof. move: DERIV; unseal => DERIV. eapply uPred.ownM_pure_soundness; eauto. Qed.
 
-  Lemma Own_general_soundness x P (VALID : ✓ x) (DERIV : Own x ⊢ P) : uPred_holds P x.
+  Lemma Own_general_soundness a P (VALID : ✓ a) (DERIV : Own a ⊢ P) : uPred_holds P a.
   Proof. move: DERIV; unseal=> DERIV; eapply uPred.ownM_general_soundness; eauto. Qed.
 
-  Lemma Own_general_completeness x P (HOLDS : uPred_holds P x) : Own x ⊢ P.
+  Lemma Own_general_completeness a P (HOLDS : uPred_holds P a) : Own a ⊢ P.
   Proof. split; unseal; uPred.unseal; i; eapply uPred_mono; eauto. Qed.
 
-  Global Instance into_sep_own (a b1 b2 : Σ) :
+  Global Instance into_sep_Own (a b1 b2 : Σ) :
     IsOp a b1 b2 → IntoSep (Own a) (Own b1) (Own b2).
   Proof. intros. by rewrite /IntoSep (is_op a) Own_op. Qed.
 
-  Global Instance into_and_own p (a b1 b2 : Σ) :
+  Global Instance into_and_Own p (a b1 b2 : Σ) :
     IsOp a b1 b2 → IntoAnd p (Own a) (Own b1) (Own b2).
   Proof. intros. by rewrite /IntoAnd (is_op a) Own_op bi.sep_and. Qed.
 
-  Global Instance from_sep_own (a b1 b2 : Σ) :
+  Global Instance from_sep_Own (a b1 b2 : Σ) :
     IsOp a b1 b2 →
     FromSep (Own a) (Own b1) (Own b2).
   Proof. intros. by rewrite /FromSep -Own_op -is_op. Qed.
@@ -432,18 +360,18 @@ Section class_instances.
   (* TODO : Improve this instance with generic own simplification machinery
   once https://gitlab.mpi-sws.org/iris/iris/-/issues/460 is fixed *)
   (* Cost > 50 to give priority to [combine_sep_as_fractional]. *)
-  Global Instance combine_sep_as_own (a b1 b2 : Σ) :
+  Global Instance combine_sep_as_Own (a b1 b2 : Σ) :
     IsOp a b1 b2 → CombineSepAs (Own b1) (Own b2) (Own a) | 60.
   Proof. intros. by rewrite /CombineSepAs -Own_op -is_op. Qed.
   (* TODO : Improve this instance with generic own validity simplification
   machinery once https://gitlab.mpi-sws.org/iris/iris/-/issues/460 is fixed *)
-  Global Instance combine_sep_gives_own (b1 b2 : Σ) :
+  Global Instance combine_sep_gives_Own (b1 b2 : Σ) :
     CombineSepGives (Own b1) (Own b2) (⌜✓ (b1 ⋅ b2)⌝).
   Proof.
     intros. rewrite /CombineSepGives -Own_op Own_valid.
     by apply : bi.persistently_intro.
   Qed.
-  Global Instance from_and_own_persistent (a b1 b2 : Σ) :
+  Global Instance from_and_Own_persistent (a b1 b2 : Σ) :
     IsOp a b1 b2 → TCOr (CoreId b1) (CoreId b2) →
     FromAnd (Own a) (Own b1) (Own b2).
   Proof.
@@ -451,120 +379,4 @@ Section class_instances.
     destruct Hb; by rewrite bi.persistent_and_sep.
   Qed.
 
-  Lemma OwnM_op (M : ucmra) `{@GRA.inG M Σ} (a1 a2 : M) :
-    (OwnM (a1 ⋅ a2)) ⊣⊢ (OwnM a1 ∗ OwnM a2).
-  Proof. by rewrite /OwnM -GRA.embed_add Own_op. Qed.
-
-  Global Instance OwnM_ne `{@GRA.inG M Σ} : NonExpansive (@OwnM Σ M _).
-  Proof. solve_proper. Qed.
-  Global Instance OwnM_proper (M : ucmra) `{@GRA.inG M Σ} :
-    Proper ((≡) ==> (⊣⊢)) (@OwnM Σ M _) := ne_proper _.
-
-  Global Instance OwnM_core_persistent `{@GRA.inG M Σ} (a : M) :
-    CoreId a → Persistent (OwnM a).
-  Proof.
-    rewrite /OwnM => CORE. apply Own_core_persistent.
-    rewrite core_id_total -GRA.embed_core core_id_core //.
-  Qed.
-
-  Lemma OwnM_valid (M : ucmra) `{@GRA.inG M Σ} (m : M):
-    OwnM m ⊢ ⌜✓ m⌝.
-  Proof.
-    iIntros "H". iDestruct (Own_valid with "H") as %WF.
-    iPureIntro. eapply GRA.embed_wf. done.
-  Qed.
-
-
-  Global Instance into_sep_ownM (M : ucmra) `{@GRA.inG M Σ} (a b1 b2 : M) :
-    IsOp a b1 b2 → IntoSep (OwnM a) (OwnM b1) (OwnM b2).
-  Proof. intros. by rewrite /IntoSep (is_op a) OwnM_op. Qed.
-
-  Global Instance into_and_ownM (M : ucmra) `{@GRA.inG M Σ} p (a b1 b2 : M) :
-    IsOp a b1 b2 → IntoAnd p (OwnM a) (OwnM b1) (OwnM b2).
-  Proof. intros. by rewrite /IntoAnd (is_op a) OwnM_op bi.sep_and. Qed.
-
-  Global Instance from_sep_ownM (M : ucmra) `{@GRA.inG M Σ} (a b1 b2 : M) :
-    IsOp a b1 b2 →
-    FromSep (OwnM a) (OwnM b1) (OwnM b2).
-  Proof. intros. by rewrite /FromSep -OwnM_op -is_op. Qed.
-
-  (* TODO : Improve this instance with generic own simplification machinery
-  once https://gitlab.mpi-sws.org/iris/iris/-/issues/460 is fixed *)
-  (* Cost > 50 to give priority to [combine_sep_as_fractional]. *)
-  Global Instance combine_sep_as_ownM (M : ucmra) `{@GRA.inG M Σ} (a b1 b2 : M) :
-    IsOp a b1 b2 → CombineSepAs (OwnM b1) (OwnM b2) (OwnM a) | 60.
-  Proof. intros. by rewrite /CombineSepAs -OwnM_op -is_op. Qed.
-  (* TODO : Improve this instance with generic own validity simplification
-  machinery once https://gitlab.mpi-sws.org/iris/iris/-/issues/460 is fixed *)
-  Global Instance combine_sep_gives_ownM (M : ucmra) `{@GRA.inG M Σ} (b1 b2 : M) :
-    CombineSepGives (OwnM b1) (OwnM b2) (⌜✓ (b1 ⋅ b2)⌝).
-  Proof.
-    intros. rewrite /CombineSepGives -OwnM_op OwnM_valid.
-    by apply : bi.persistently_intro.
-  Qed.
-  Global Instance from_and_ownM_persistent (M : ucmra) `{@GRA.inG M Σ} (a b1 b2 : M) :
-    IsOp a b1 b2 → TCOr (CoreId b1) (CoreId b2) →
-    FromAnd (OwnM a) (OwnM b1) (OwnM b2).
-  Proof.
-    intros ? Hb. rewrite /FromAnd (is_op a) OwnM_op.
-    destruct Hb; by rewrite bi.persistent_and_sep.
-  Qed.
-
-End class_instances.
-
-
-
-Section ILEMMAS.
-  Context `{Σ : GRA.t}.
-
-
-  Lemma Own_extends
-        (a b : Σ)
-        (EXT : a ≼ b)
-    :
-      Own b ⊢ Own a
-  .
-  Proof. unseal. apply uPred.ownM_mono. done. Qed.
-
-  Lemma Own_persistently (r : Σ) : Own r ⊢ <pers> Own (core r).
-  Proof. unseal. apply uPred.persistently_ownM_core. Qed.
-
-  Lemma OwnM_persistently {M : ucmra} `{@GRA.inG M Σ} (r : M) : OwnM r ⊢ <pers> OwnM (core r).
-  Proof. rewrite /OwnM GRA.embed_core Own_persistently //. Qed.
-
-  Lemma Own_unit : ⊢ Own (Σ:=Σ) ε.
-  Proof. unseal. rewrite /bi_emp_valid. apply (uPred.ownM_unit emp). Qed.
-
-  Lemma OwnM_unit {M : ucmra} `{@GRA.inG M Σ} : ⊢ OwnM ε.
-  Proof. rewrite /OwnM GRA.embed_unit. apply Own_unit. Qed.
-
-  Lemma OwnM_Upd `{M : ucmra} `{@GRA.inG M Σ}
-        (r1 r2 : M)
-        (UPD : r1 ~~> r2)
-    :
-      (OwnM r1) ⊢ (|==> (OwnM r2))
-  .
-  Proof. apply Own_Upd, GRA.embed_updatable, UPD. Qed.
-
-  Lemma OwnM_extends `{M : ucmra} `{@GRA.inG M Σ}
-        {a b : M}
-        (EXT : a ≼ b)
-    :
-      OwnM b ⊢ OwnM a
-  .
-  Proof. revert EXT. move=> [c ->]. by rewrite OwnM_op bi.sep_elim_l. Qed.
-End ILEMMAS.
-
-(* TODO : Move this to tactics *)
-Ltac iOwnWf' H :=
-  iPoseProof (OwnM_valid with H) as "%".
-
-Tactic Notation "iOwnWf" constr(H) :=
-  iOwnWf' H.
-
-Tactic Notation "iOwnWf" constr(H) "as" ident(WF) :=
-  iOwnWf' H;
-  match goal with
-  | H0 : @valid _ _ _ |- _ => rename H0 into WF
-  end
-. *)
+End Own.
