iris_system/sWorld.v
@@ -2,218 +2,221 @@ From stdpp Require Import coPset gmap namespaces.
 Require Import sflib.
 From iris Require Import bi.big_op.
 Require Import Coq.Logic.ClassicalEpsilon.
+Require Export World.
 
-Require Import Coqlib PCM IPM SRF sProp World.
+(* TODO : move these to separate files *)
 Local Notation univ_id := positive.
 Local Notation level := nat.
 
-Module WD.
+Section syn_inv.
+  Context `{!CtxSL.t Σ Γ α β τ, !invGSΓ Γ}.
 
-  Section WD.
+  Variant syn_inv_shape : Type :=
+  | _ownI (u : univ_id) (i : positive)
+  | _ownI_auth (u : univ_id) (keys : gset positive) (* TODO : gsets? *)
+  | _wsat_auth (u : univ_id) (n)
+  (* | _free_worlds (u : univ_id) (b : level) *)
+  (* | _empty_universes (eu : univ_id) *)
+  .
 
-    Context `{!CtxSL.t Σ Γ α β τ}.
-    Context `{_W0 : @GRA.inG OwnIRA Σ}.
-    Context `{_W1 : @GRA.inG OwnERA Γ}.
-    Context `{_W2 : @GRA.inG OwnDRA Γ}.
-    Notation iProp := (iProp Σ).
+  Definition inv_degree (s : inv_shape) (sProp : Type) : Type :=
+    match s with
+    (* | _OwnI u i => fin 1
+    | _OwnI_auth u keys => positive
+    | _free_worlds u b => fin 0
+    | _empty_universes u => fin 0 *)
+    | _inv u n N p => fin 0
+    | _wsats u n E => fin 0
+    end.
 
-    Variant shape : Type :=
-    | _OwnI (u : univ_id) (i : positive)
-    | _OwnI_auth (u : univ_id) (keys : list positive) (* TODO : gsets? *)
-    | _free_worlds (u : univ_id) (b : level)
-    | _empty_universes (eu : univ_id)
-    .
-
-    Definition degree (s : shape) (sProp : Type) : Type :=
-      match s with
-      | _OwnI u i => fin 1
-      | _OwnI_auth u keys => positive
-      | _free_worlds u b => fin 0
-      | _empty_universes u => fin 0
-      end.
-
-    Global Instance syntax : PF.t := {
-        shp := shape;
-        deg := degree;
-      }.
-
-    Definition interp n (s : shape)
-        : (degree s (SRFSyn.t_prev n) → SRFSyn.t n) → (degree s (SRFSyn.t_prev n) → iProp) → iProp :=
-      match s with
-      | _OwnI u i => fun syn _ =>
-          OwnI u n i (syn 0%fin)
-      | _OwnI_auth u keys => fun syn _ =>
-          OwnI_auth u n (list_to_map ((fun i => (i, syn i)) <$> keys))
-      | _free_worlds u b => fun _ _ =>
-          free_worlds u b
-      | _empty_universes eu => fun _ _ =>
-          empty_universes eu
-      end.
-
-    Global Instance t: SRFIntpM.t := interp.
-
-    Context `{_W3 : @SRFIntp.inG SL.domain syntax α t β}.
-
-    Definition OwnI u n i (p : SRFSyn.t n) : SRFSyn.t n :=
-      ⟨ _OwnI u i, fun _ => p ⟩%SRF.
-    Definition OwnI_auth u n (I : gmap positive (SRFSyn.t n)) : SRFSyn.t n :=
-      ⟨ _OwnI_auth u (elements (dom I)), fun i => or_else (I !! i) emp⟩%SRF.
-    Definition free_worlds u b : SRFSyn.t b :=
-      ⟨ _free_worlds u b, fun e => match e with end ⟩%SRF.
-    Definition empty_universes eu {n} : SRFSyn.t n :=
-      ⟨ _empty_universes eu , fun a => match a with end ⟩%SRF.
-
-    Definition OwnE (u : univ_id) {n} (E : coPset) : SRFSyn.t n :=
-      (<ownm> (OwnER u E))%SRF.
-    Definition OwnD (u : univ_id) {n} (D : gset positive) : SRFSyn.t n :=
-      (<ownm> (OwnDR u D))%SRF.
-    Definition ownD_auth (u : univ_id) {n} : SRFSyn.t n :=
-      (∃ D : τ{⇣gset positive}, <ownm> (OwnD_authR u D))%SRF.
-
-    Definition inv_satall u n (I : gmap positive (SRFSyn.t n)) : SRFSyn.t n :=
-      ([∗ n map] i ↦ p ∈ I, (p ∗ OwnD u {[i]}) ∨ OwnE u {[i]})%SRF.
-    Definition wsat u n : SRFSyn.t (S n) :=
-      (∃ I : τ{ST.gmapT Φ}, (⤉ OwnI_auth u n I) ∗ (⤉ inv_satall u n I))%SRF.
-
-    (* Definition empty_worlds (eu : univ_id) {n} : SRFSyn.t n := *)
-      (* (<ownm> (empty_worldsR eu (fun _ => Some ⊤ : CoPset.t) : OwnERA) ∗ *)
-      (* <ownm> (empty_worldsR eu (fun _ => Auth.black (Some ∅ : Gset.t)) : OwnDRA) ∗ *)
-      (* ownI_free eu). *)
-    Definition free_universes {n} : SRFSyn.t n :=
-      (∃ eu : τ{⇣ univ_id}, empty_universes eu)%SRF.
-    Fixpoint wsats u b : SRFSyn.t b :=
-      match b with
-      | 0 => emp%SRF
-      | S n => (wsat u n ∗ ⤉ wsats u n)%SRF
-      end.
-
-    (* Interface for the user *)
-    Definition used_worlds u b E : SRFSyn.t b :=
-      wsats u b ∗ OwnE u E ∗ ownD_auth u ∗ free_universes.
-    Definition closed_universe u b E : SRFSyn.t b :=
-      used_worlds u b E ∗ free_worlds u b.
-    Definition inv u (n : level) (N : namespace) p :=
-      (∃ i : τ{⇣positive}, ⌜i ∈ (↑N : coPset)⌝ ∧ OwnI u n i p)%SRF.
-    Definition FUpd u b (A : SRFSyn.t b) (E1 E2 : coPset) (P : SRFSyn.t b) : SRFSyn.t b :=
-      A ∗ used_worlds u b E1 -∗ |==> (A ∗ used_worlds u b E2 ∗ P).
-
-  End WD.
-
-End WD.
-
-Module Inv.
-
-  Class t Σ Γ α β τ :=
-    { #[global] ctxSL :: CtxSL.t Σ Γ α β τ;
-      #[global] IinG :: @GRA.inG OwnIRA Σ;
-      #[global] EinG :: @GRA.inG OwnERA Γ;
-      #[global] DinG :: @GRA.inG OwnDRA Γ;
-      #[global] IntpG :: @SRFIntp.inG SL.domain WD.syntax α WD.t β
+  Global Instance inv_syntax : PF.t := {
+      shp := inv_shape;
+      deg := inv_degree;
     }.
 
-End Inv.
+  Definition inv_interp_aux n (s : inv_shape)
+      : (inv_degree s (SRFSyn.t_prev n) → SRFSyn.t n) → (inv_degree s (SRFSyn.t_prev n) → iProp Σ)
+        → iProp Σ :=
+    match s with
+    (* | _OwnI u i => fun syn _ =>
+        OwnI u n i (syn 0%fin)
+    | _OwnI_auth u keys => fun syn _ =>
+        OwnI_auth u n (list_to_map ((fun i => (i, syn i)) <$> keys))
+    | _free_worlds u b => fun _ _ =>
+        free_worlds u b
+    | _empty_universes eu => fun _ _ =>
+        empty_universes eu *)
+    | _inv u n N p => λ _ _, inv u n N p
+    | _wsats u n E => λ _ _, wsats u n E
+    end.
 
-Module WDRed.
+  Global Instance inv_interp : SRFIntpM.t := inv_interp_aux.
 
-  Section RED.
+  Context `{_W3 : @SRFIntp.inG SL.domain inv_syntax α inv_interp β}.
 
-    Context `{_C : Inv.t}.
+  (* Definition OwnI u n i (p : SRFSyn.t n) : SRFSyn.t n := *)
+    (* ⟨ _OwnI u i, fun _ => p ⟩%SRF. *)
+  (* Definition OwnI_auth u n (I : gmap positive (SRFSyn.t n)) : SRFSyn.t n := *)
+    (* ⟨ _OwnI_auth u (elements (dom I)), fun i => or_else (I !! i) emp⟩%SRF. *)
+  (* Definition free_worlds u b : SRFSyn.t b := *)
+    (* ⟨ _free_worlds u b, fun e => match e with end ⟩%SRF. *)
+  (* Definition empty_universes eu {n} : SRFSyn.t n := *)
+    (* ⟨ _empty_universes eu , fun a => match a with end ⟩%SRF. *)
 
-    Lemma OwnI_auth u n I  :
-      SRFSem.t n (WD.OwnI_auth u n I) = OwnI_auth u n I.
-    Proof.
-      rewrite /WD.OwnI_auth. SRF_red_all. ss.
-      rewrite /OwnI_auth /OwnI_authR; do 5 f_equal.
-      apply map_eq; intros i.
-      destruct (I !! i) eqn : EI; rewrite EI.
-      { rewrite -elem_of_list_to_map.
-        rewrite elem_of_list_fmap; exists i; rewrite EI; ss; split; eauto;
-          by rewrite elem_of_elements elem_of_dom; rewrite EI.
-        eapply NoDup_fmap_fst.
-        { intros ???. rewrite !elem_of_list_fmap; ii; des; clarify. }
-        eapply NoDup_fmap_2; last by eapply NoDup_elements.
-        ii; clarify.
-      }
-      { eapply not_elem_of_list_to_map_1; intros H.
-        rewrite elem_of_list_fmap in H; des; clarify.
-        eapply elem_of_list_fmap_2 in H0; des; clarify; ss.
-        rewrite elem_of_elements elem_of_dom in H1; rewrite EI in H1; ss; inv H1.
-      }
-    Qed.
+  (* Definition OwnE (u : univ_id) {n} (E : coPset) : SRFSyn.t n := *)
+    (* (<ownm> (OwnER u E))%SRF. *)
+  (* Definition OwnD (u : univ_id) {n} (D : gset positive) : SRFSyn.t n := *)
+    (* (<ownm> (OwnDR u D))%SRF. *)
+  (* Definition ownD_auth (u : univ_id) {n} : SRFSyn.t n := *)
+    (* (∃ D : τ{⇣gset positive}, <ownm> (OwnD_authR u D))%SRF. *)
 
-    Lemma wsat u n:
-      SRFSem.t (S n) (WD.wsat u n) ≡ wsat u n.
-    Proof.
-      rewrite /WD.wsat /wsat. SL_red.
-      rewrite bi.equiv_entails; split; ss; iIntros "[%I WD]"; SL_red; iDestruct "WD" as "[WD1 WD2]"; SL_red.
-      { SRF_red; SL_red; rewrite OwnI_auth /inv_satall; iExists I; iFrame.
-        iApply (big_sepM_impl with "WD2"); iModIntro; iIntros. rewrite /WD.OwnD /WD.OwnE; SL_red; SL_red_ownm; ss.
-      }
-      { iExists I; SL_red. SL_red. SRF_red. rewrite OwnI_auth; iFrame.
-        SL_red; rewrite /inv_satall. iApply (big_sepM_impl with "WD2"); iModIntro; iIntros. SL_red; SL_red_ownm; ss.
-      }
-    Qed.
+  (* Definition inv_satall u n (I : gmap positive (SRFSyn.t n)) : SRFSyn.t n := *)
+    (* ([∗ n map] i ↦ p ∈ I, (p ∗ OwnD u {[i]}) ∨ OwnE u {[i]})%SRF. *)
+  (* Definition wsat u n : SRFSyn.t (S n) := *)
+    (* (∃ I : τ{ST.gmapT Φ}, (⤉ OwnI_auth u n I) ∗ (⤉ inv_satall u n I))%SRF. *)
+  Definition syn_wsats (u : univ_id) (n : level) (E : coPset) : SRFSyn.t n :=
+    ⟨ _wsats u n E, λ e, match e with end ⟩%SRF.
+  Definition syn_inv (u : univ_id) (n : level) (N : namespace) (p : SRFSyn.t n) : SRFSyn.t n :=
+    ⟨ _inv u n N p, λ e, match e with end ⟩%SRF.
+  (* Definition syn_fupd u b (E1 E2 : coPset) (P : iProp Σ) : SRFSyn.t n :=
+    syn_wsats u b E1 ==∗ (syn_wsats u b E2 ∗ P) *)
 
-    Lemma wsats u b:
-      SRFSem.t b (WD.wsats u b) ≡ wsats u b.
-    Proof.
-      induction b; ss.
-      - SL_red. eauto.
-      - rewrite @SLRed.sepconj wsat. SRF_red. rewrite IHb. by rewrite wsats_fold.
-    Qed.
+  (* Definition empty_worlds (eu : univ_id) {n} : SRFSyn.t n := *)
+    (* (<ownm> (empty_worldsR eu (fun _ => Some ⊤ : CoPset.t) : OwnERA) ∗ *)
+    (* <ownm> (empty_worldsR eu (fun _ => Auth.black (Some ∅ : Gset.t)) : OwnDRA) ∗ *)
+    (* ownI_free eu). *)
+  (* Definition free_universes {n} : SRFSyn.t n :=
+    (∃ eu : τ{⇣ univ_id}, empty_universes eu)%SRF.
+  Fixpoint wsats u b : SRFSyn.t b :=
+    match b with
+    | 0 => emp%SRF
+    | S n => (wsat u n ∗ ⤉ wsats u n)%SRF
+    end. *)
+
+  (* Interface for the user *)
+  (* Definition used_worlds u b E : SRFSyn.t b := *)
+    (* wsats u b ∗ OwnE u E ∗ ownD_auth u ∗ free_universes. *)
+  (* Definition closed_universe u b E : SRFSyn.t b := *)
+    (* used_worlds u b E ∗ free_worlds u b. *)
+  (* Definition inv u (n : level) (N : namespace) p := *)
+    (* (∃ i : τ{⇣positive}, ⌜i ∈ (↑N : coPset)⌝ ∧ OwnI u n i p)%SRF. *)
+  (* Definition FUpd u b (A : SRFSyn.t b) (E1 E2 : coPset) (P : SRFSyn.t b) : SRFSyn.t b := *)
+    (* A ∗ used_worlds u b E1 -∗ |==> (A ∗ used_worlds u b E2 ∗ P). *)
+  Context (p : SRFSyn.t 0).
+  Check (syn_inv 1 0 nil (syn_wsats 1 0 ⊤)).
+End syn_inv.
+
+Class sinvGS Σ Γ α β τ :=
+  { #[global] sinv_CtxSL :: CtxSL.t Σ Γ α β τ;
+    #[global] sinv_invGS :: invGS Σ Γ;
+    #[global] sinv_intpG :: @SRFIntp.inG SL.domain inv_syntax α inv_interp β
+  }.
+
+Module WDRed. Section RED.
+  Context `{!sinvGS Σ Γ α β τ}.
+
+  Lemma wsats u n E : ⟦syn_wsats u n E⟧ = wsats u n E.
+  Proof. rewrite /syn_wsats. SRF_red_all. ss. Qed.
+  Lemma inv u n N p : ⟦syn_inv u n N p⟧ = inv u n N p.
+  Proof. rewrite /syn_inv. SRF_red_all. ss. Qed.
+
+    (* Context `{_C : Inv.t}. *)
+
+    (* Lemma OwnI_auth u n I  : *)
+      (* SRFSem.t n (WD.OwnI_auth u n I) = OwnI_auth u n I. *)
+    (* Proof. *)
+      (* rewrite /WD.OwnI_auth. SRF_red_all. ss. *)
+      (* rewrite /OwnI_auth /OwnI_authR; do 5 f_equal. *)
+      (* apply map_eq; intros i. *)
+      (* destruct (I !! i) eqn : EI; rewrite EI. *)
+      (* { rewrite -elem_of_list_to_map. *)
+        (* rewrite elem_of_list_fmap; exists i; rewrite EI; ss; split; eauto; *)
+          (* by rewrite elem_of_elements elem_of_dom; rewrite EI. *)
+        (* eapply NoDup_fmap_fst. *)
+        (* { intros ???. rewrite !elem_of_list_fmap; ii; des; clarify. } *)
+        (* eapply NoDup_fmap_2; last by eapply NoDup_elements. *)
+        (* ii; clarify. *)
+      (* } *)
+      (* { eapply not_elem_of_list_to_map_1; intros H. *)
+        (* rewrite elem_of_list_fmap in H; des; clarify. *)
+        (* eapply elem_of_list_fmap_2 in H0; des; clarify; ss. *)
+        (* rewrite elem_of_elements elem_of_dom in H1; rewrite EI in H1; ss; inv H1. *)
+      (* } *)
+    (* Qed. *)
+
+    (* Lemma wsat u n: *)
+      (* SRFSem.t (S n) (WD.wsat u n) ≡ wsat u n. *)
+    (* Proof. *)
+      (* rewrite /WD.wsat /wsat. SL_red. *)
+      (* rewrite bi.equiv_entails; split; ss; iIntros "[%I WD]"; SL_red; iDestruct "WD" as "[WD1 WD2]"; SL_red. *)
+      (* { SRF_red; SL_red; rewrite OwnI_auth /inv_satall; iExists I; iFrame. *)
+        (* iApply (big_sepM_impl with "WD2"); iModIntro; iIntros. rewrite /WD.OwnD /WD.OwnE; SL_red; SL_red_ownm; ss. *)
+      (* } *)
+      (* { iExists I; SL_red. SL_red. SRF_red. rewrite OwnI_auth; iFrame. *)
+        (* SL_red; rewrite /inv_satall. iApply (big_sepM_impl with "WD2"); iModIntro; iIntros. SL_red; SL_red_ownm; ss. *)
+      (* } *)
+    (* Qed. *)
+
+    (* Lemma wsats u b: *)
+      (* SRFSem.t b (WD.wsats u b) ≡ wsats u b. *)
+    (* Proof. *)
+      (* induction b; ss. *)
+      (* - SL_red. eauto. *)
+      (* - rewrite @SLRed.sepconj wsat. SRF_red. rewrite IHb. by rewrite wsats_fold. *)
+    (* Qed. *)
 
     (* User Interface *)
-    Lemma used_worlds u b E :
-      SRFSem.t b (WD.used_worlds u b E) ≡ used_worlds u b E.
-    Proof.
-      SL_red; rewrite wsats; rewrite bi.equiv_entails; split.
-      { iIntros "[WSAT [E [[% D] [% U]]]]"; SL_red; iFrame.
-        by rewrite /WD.empty_universes; SRF_red; SL_red_ownm; ss; iFrame. }
-      { iIntros "[WSAT [E [[% D] [% U]]]]"; SL_red; SL_red_ownm; iFrame.
-        iSplitL "D"; [iExists D|iExists eu]; last by rewrite /WD.empty_universes; SRF_red; ss; iFrame.
-        SL_red; SL_red_ownm; iFrame.
-      }
-    Qed.
+    (* Lemma used_worlds u b E : *)
+      (* SRFSem.t b (WD.used_worlds u b E) ≡ used_worlds u b E. *)
+    (* Proof. *)
+      (* SL_red; rewrite wsats; rewrite bi.equiv_entails; split. *)
+      (* { iIntros "[WSAT [E [[% D] [% U]]]]"; SL_red; iFrame. *)
+        (* by rewrite /WD.empty_universes; SRF_red; SL_red_ownm; ss; iFrame. } *)
+      (* { iIntros "[WSAT [E [[% D] [% U]]]]"; SL_red; SL_red_ownm; iFrame. *)
+        (* iSplitL "D"; [iExists D|iExists eu]; last by rewrite /WD.empty_universes; SRF_red; ss; iFrame. *)
+        (* SL_red; SL_red_ownm; iFrame. *)
+      (* } *)
+    (* Qed. *)
 
-    Lemma free_worlds u b :
-      SRFSem.t b (WD.free_worlds u b) = free_worlds u b.
-    Proof.
-      unfold free_worlds, WD.free_worlds. SRF_red. eauto.
-    Qed.
+    (* Lemma free_worlds u b : *)
+      (* SRFSem.t b (WD.free_worlds u b) = free_worlds u b. *)
+    (* Proof. *)
+      (* unfold free_worlds, WD.free_worlds. SRF_red. eauto. *)
+    (* Qed. *)
 
-    Lemma closed_universe u b E :
-      SRFSem.t b (WD.closed_universe u b E) ≡ closed_universe u b E.
-    Proof.
-      rewrite /WD.closed_universe /closed_universe @SLRed.sepconj used_worlds free_worlds; ss.
-    Qed.
+    (* Lemma closed_universe u b E : *)
+      (* SRFSem.t b (WD.closed_universe u b E) ≡ closed_universe u b E. *)
+    (* Proof. *)
+      (* rewrite /WD.closed_universe /closed_universe @SLRed.sepconj used_worlds free_worlds; ss. *)
+    (* Qed. *)
 
-    Lemma inv u n N p :
-      SRFSem.t n (WD.inv u n N p) ≡ inv u n N p.
-    Proof.
-      rewrite /WD.inv /inv; SL_red; rewrite bi.equiv_entails; split; iIntros "[%x H]"; SL_red.
-      { iExists x; rewrite /WD.OwnI; SRF_red; ss. }
-      { iExists x; SL_red; rewrite /WD.OwnI; SRF_red; ss. }
-    Qed.
+    (* Lemma inv u n N p : *)
+      (* SRFSem.t n (WD.inv u n N p) ≡ inv u n N p. *)
+    (* Proof. *)
+      (* rewrite /WD.inv /inv; SL_red; rewrite bi.equiv_entails; split; iIntros "[%x H]"; SL_red. *)
+      (* { iExists x; rewrite /WD.OwnI; SRF_red; ss. } *)
+      (* { iExists x; SL_red; rewrite /WD.OwnI; SRF_red; ss. } *)
+    (* Qed. *)
 
-    Lemma FUpd u b A E1 E2 P :
-      SRFSem.t b (WD.FUpd u b A E1 E2 P) ≡ FUpd u b ⟦A⟧ E1 E2 ⟦P⟧.
-    Proof.
-      Local Transparent FUpd.
-      unfold WD.FUpd, FUpd. rewrite !@SLRed.wand !@SLRed.upd @SLRed.sepconj. rewrite -> used_worlds.
-      do 2 rewrite @SLRed.sepconj. rewrite used_worlds. eauto.
-    Qed.
+    (* Lemma FUpd u b A E1 E2 P : *)
+      (* SRFSem.t b (WD.FUpd u b A E1 E2 P) ≡ FUpd u b ⟦A⟧ E1 E2 ⟦P⟧. *)
+    (* Proof. *)
+      (* Local Transparent FUpd. *)
+      (* unfold WD.FUpd, FUpd. rewrite !@SLRed.wand !@SLRed.upd @SLRed.sepconj. rewrite -> used_worlds. *)
+      (* do 2 rewrite @SLRed.sepconj. rewrite used_worlds. eauto. *)
+    (* Qed. *)
 
   End RED.
 End WDRed.
 
-Global Opaque WD.used_worlds.
-Global Opaque WD.free_worlds.
-Global Opaque WD.inv.
-Global Opaque WD.FUpd.
-Global Opaque used_worlds.
-Global Opaque free_worlds.
-Global Opaque inv.
-Global Opaque FUpd.
+(* Global Opaque WD.used_worlds. *)
+(* Global Opaque WD.free_worlds. *)
+(* Global Opaque WD.inv. *)
+(* Global Opaque WD.FUpd. *)
+(* Global Opaque used_worlds. *)
+(* Global Opaque free_worlds. *)
+(* Global Opaque inv. *)
+(* Global Opaque FUpd. *)
 
 
 Ltac WD_red := repeat (
