simulations/isim/ISim.v
@@ -37,7 +37,7 @@ End LEMMAS.
 
 Section HModProd.
 
-  Context `{Σ : GRA.t}.
+  Context `{Σ : GRA}.
   Notation iProp := (iProp Σ).
 
   Definition IstProd0 (IstL IstR : nat -> alist key Any.t -> alist key Any.t -> iProp) :=
